matching-logic/src/ProofMode_fixpoint.v
@@ -14,6 +14,7 @@ From MatchingLogic Require Import
     ProofSystem
     IndexManipulation
     wftactics
+    ProofInfo
     ProofMode_base
     ProofMode_propositional
 .
@@ -36,28 +37,6 @@ Set Default Proof Mode "Classic".
 Open Scope ml_scope.
 Open Scope string_scope.
 Open Scope list_scope.
-
-
-Lemma pile_impl_uses_kt {Σ : Signature} gpi evs svs fp:
-  ProofInfoLe ( (ExGen := evs, SVSubst := svs, KT := true, FP := fp)) ( gpi) ->
-  pi_uses_kt gpi.
-Proof.
-  intros [H].
-  specialize (H ∅).
-  pose (pf1 := @A_impl_A Σ ∅ patt_bott ltac:(wf_auto2)).
-  pose (pf2 := @ProofSystem.Knaster_tarski Σ ∅ (patt_bound_svar 0) patt_bott ltac:(wf_auto2) (proj1_sig pf1)).
-  specialize (H _ pf2).
-  feed specialize H.
-  {
-    constructor; simpl.
-    { set_solver. }
-    { set_solver. }
-    reflexivity.
-    { clear. set_solver. }
-  }
-  destruct H as [H1 H2 H3 H4].
-  unfold pf2 in H3. simpl in H3. exact H3.
-Qed.
 
 
 Lemma Knaster_tarski {Σ : Signature}
@@ -92,7 +71,7 @@ unshelve (eexists).
   }
   {
     destruct Hpf as [Hpf2 Hpf3 Hpf4].
-    pose proof (Hpile := @pile_impl_uses_kt _ _ _ _ _ pile).
+    pose proof (Hpile := pile_impl_uses_kt _ _ _ _ pile).
     exact Hpile.
   }
   {
@@ -101,28 +80,6 @@ unshelve (eexists).
   }
 }
 Defined.
-
-Lemma pile_impl_allows_svsubst_X {Σ : Signature} gpi evs X kt fp:
-  ProofInfoLe ( (ExGen := evs, SVSubst := {[X]}, KT := kt, FP := fp)) ( gpi) ->
-  X ∈ pi_substituted_svars gpi.
-Proof.
-  intros [H].
-  specialize (H ∅).
-  pose (pf1 := @A_impl_A Σ ∅ (patt_free_svar X) ltac:(wf_auto2)).
-  pose (pf2 := @ProofSystem.Svar_subst Σ ∅ (patt_free_svar X ---> patt_free_svar X) patt_bott X ltac:(wf_auto2) ltac:(wf_auto2) (proj1_sig pf1)).
-  specialize (H _ pf2).
-  feed specialize H.
-  {
-    constructor; simpl.
-    { set_solver. }
-    { set_solver. }
-    reflexivity.
-    { clear. set_solver. }
-  }
-  destruct H as [H1 H2 H3 H4].
-  simpl in *.
-  clear -H2. set_solver.
-Qed.
 
 Lemma Svar_subst {Σ : Signature}
   (Γ : Theory) (ϕ ψ : Pattern) (X : svar)  (i : ProofInfo)
@@ -140,7 +97,7 @@ Proof.
   unshelve (eexists).
   {
    apply ProofSystem.Svar_subst.
-   { pose proof (Hwf := @proved_impl_wf _ _ _ pf). exact Hwf. }
+   { pose proof (Hwf := proved_impl_wf _ _ pf). exact Hwf. }
    { exact wfψ. }
    { exact pf. }
   }
@@ -153,7 +110,7 @@ Proof.
   }
   {
     destruct Hpf as [Hpf2 Hpf3 Hpf4].
-    pose proof (Hpile := @pile_impl_allows_svsubst_X _ _ _ _ _ _ pile).
+    pose proof (Hpile := pile_impl_allows_svsubst_X _ _ _ _ _ pile).
     clear -Hpile Hpf3.
     set_solver.
   }
@@ -190,149 +147,149 @@ Proof.
   }
 Defined.
 
-  Lemma mu_monotone {Σ : Signature} Γ ϕ₁ ϕ₂ X (i : ProofInfo):
-    ProofInfoLe ( (ExGen := ∅, SVSubst := {[X]}, KT := true, FP := ∅)) i ->
-    svar_has_negative_occurrence X ϕ₁ = false ->
-    svar_has_negative_occurrence X ϕ₂ = false ->
-    Γ ⊢i ϕ₁ ---> ϕ₂ using i->
-    Γ ⊢i (patt_mu (ϕ₁^{{svar: X ↦ 0}})) ---> (patt_mu (ϕ₂^{{svar: X ↦ 0}}))
-    using i.
-  Proof.
-    intros pile nonegϕ₁ nonegϕ₂ Himp.
-    pose proof (wfϕ12 := @proved_impl_wf _ _ _ (proj1_sig Himp)).
-    assert(wfϕ₁ : well_formed ϕ₁) by wf_auto2.
-    assert(wfϕ₂ : well_formed ϕ₂) by wf_auto2.
+Lemma mu_monotone {Σ : Signature} Γ ϕ₁ ϕ₂ X (i : ProofInfo):
+  ProofInfoLe ( (ExGen := ∅, SVSubst := {[X]}, KT := true, FP := ∅)) i ->
+  svar_has_negative_occurrence X ϕ₁ = false ->
+  svar_has_negative_occurrence X ϕ₂ = false ->
+  Γ ⊢i ϕ₁ ---> ϕ₂ using i->
+  Γ ⊢i (patt_mu (ϕ₁^{{svar: X ↦ 0}})) ---> (patt_mu (ϕ₂^{{svar: X ↦ 0}}))
+  using i.
+Proof.
+  intros pile nonegϕ₁ nonegϕ₂ Himp.
+  pose proof (wfϕ12 := proved_impl_wf _ _ (proj1_sig Himp)).
+  assert(wfϕ₁ : well_formed ϕ₁) by wf_auto2.
+  assert(wfϕ₂ : well_formed ϕ₂) by wf_auto2.
 
-    apply Knaster_tarski.
-    { eapply pile_trans. 2: apply pile. apply pile_svs_subseteq. set_solver. }
-    { wf_auto2. }
+  apply Knaster_tarski.
+  { eapply pile_trans. 2: apply pile. apply pile_svs_subseteq. set_solver. }
+  { wf_auto2. }
 
-    pose proof (Htmp := @Svar_subst Σ Γ (ϕ₁ ---> ϕ₂) (mu, ϕ₂^{{svar: X ↦ 0}}) X i).
-    feed specialize Htmp.
-    { eapply pile_trans. 2: apply pile. apply pile_kt_impl. simpl. reflexivity. }
-    { wf_auto2. }
-    { exact Himp. }
-    unfold free_svar_subst in Htmp.
-    simpl in Htmp.
-    fold free_svar_subst in Htmp.
+  pose proof (Htmp := @Svar_subst Σ Γ (ϕ₁ ---> ϕ₂) (mu, ϕ₂^{{svar: X ↦ 0}}) X i).
+  feed specialize Htmp.
+  { eapply pile_trans. 2: apply pile. apply pile_kt_impl. simpl. reflexivity. }
+  { wf_auto2. }
+  { exact Himp. }
+  unfold free_svar_subst in Htmp.
+  simpl in Htmp.
+  fold free_svar_subst in Htmp.
 
-    pose proof (Hpf := @Pre_fixp Σ Γ (ϕ₂^{{svar: X ↦ 0}})).
-    simpl in Hpf.
+  pose proof (Hpf := Pre_fixp Γ (ϕ₂^{{svar: X ↦ 0}})).
+  simpl in Hpf.
 
-    unshelve (eapply (@cast_proof' Σ Γ _ _) in Hpf).
-    3: { 
-    erewrite bound_to_free_set_variable_subst.
-      5: { apply svar_quantify_not_free. }
-      4: {
+  unshelve (eapply (cast_proof' Γ _ _) in Hpf).
+  3: { 
+  erewrite bound_to_free_set_variable_subst.
+    5: { apply svar_quantify_not_free. }
+    4: {
+     apply svar_quantify_closed_mu.
+     unfold well_formed, well_formed_closed in *. destruct_and!. auto.
+    }
+    3: {
        apply svar_quantify_closed_mu.
        unfold well_formed, well_formed_closed in *. destruct_and!. auto.
-      }
-      3: {
+    }
+    2: lia.
+    reflexivity.
+  }
+
+  2: abstract (wf_auto2).
+
+  eapply (cast_proof' Γ) in Hpf.
+  2: {
+    rewrite svar_open_svar_quantify.
+    { unfold well_formed, well_formed_closed in *. destruct_and!. auto. }
+    reflexivity.
+  }
+
+
+  assert(well_formed_positive (ϕ₂^[[svar: X ↦ mu , ϕ₂^{{svar: X ↦ 0}}]]) = true).
+  {
+    unfold well_formed, well_formed_closed in *. destruct_and!. simpl; split_and?.
+    apply wfp_free_svar_subst; auto.
+    { apply svar_quantify_closed_mu. auto. }
+    { simpl. split_and!.
+      2: apply well_formed_positive_svar_quantify; assumption.
+      apply no_negative_occurrence_svar_quantify; auto.
+    }
+  }
+
+  assert(well_formed_closed_mu_aux (ϕ₂^[[svar: X ↦ mu , ϕ₂^{{svar: X ↦ 0}}]]) 0 = true).
+  {
+    unfold well_formed, well_formed_closed in *. destruct_and!. simpl; split_and?; auto.
+    replace 0 with (0 + 0) at 3 by lia.
+    apply wfc_mu_free_svar_subst; auto.
+    simpl.
+    apply svar_quantify_closed_mu. assumption.
+  }
+
+  assert(well_formed_closed_ex_aux (ϕ₂^[[svar: X ↦ mu , ϕ₂^{{svar: X ↦ 0}}]]) 0 = true).
+  {
+    unfold well_formed, well_formed_closed in *. destruct_and!. simpl; split_and?; auto.
+    replace 0 with (0 + 0) at 3 by lia.
+    apply wfc_ex_free_svar_subst; auto.
+    simpl.
+    apply svar_quantify_closed_ex. assumption.
+  }
+
+  assert(well_formed_positive (ϕ₁^[[svar: X ↦ mu , ϕ₂^{{svar: X ↦ 0}}]]) = true).
+  {
+    unfold well_formed, well_formed_closed in *. destruct_and!. simpl; split_and?.
+    apply wfp_free_svar_subst; auto.
+    { apply svar_quantify_closed_mu. auto. }
+    { simpl. split_and!.
+      2: apply well_formed_positive_svar_quantify; assumption.
+      apply no_negative_occurrence_svar_quantify; auto.
+    }
+  }
+
+  assert(well_formed_closed_mu_aux (ϕ₁^[[svar: X ↦ mu , ϕ₂^{{svar: X ↦ 0}}]]) 0 = true).
+  {
+    unfold well_formed, well_formed_closed in *. destruct_and!. simpl; split_and?; auto.
+    replace 0 with (0 + 0) at 3 by lia.
+    apply wfc_mu_free_svar_subst; auto.
+    simpl.
+    apply svar_quantify_closed_mu. assumption.
+  }
+
+  assert(well_formed_closed_ex_aux (ϕ₁^[[svar: X ↦ mu , ϕ₂^{{svar: X ↦ 0}}]]) 0 = true).
+  {
+    unfold well_formed, well_formed_closed in *. destruct_and!. simpl; split_and?; auto.
+    replace 0 with (0 + 0) at 3 by lia.
+    apply wfc_ex_free_svar_subst; auto.
+    simpl.
+    apply svar_quantify_closed_ex. assumption.
+  }
+
+  apply useBasicReasoning with (i := i) in Hpf.
+  epose proof (Hsi := syllogism_meta _ _ _ Htmp Hpf).
+  simpl.
+
+  eapply (@cast_proof' Σ Γ).
+  1: {
+    erewrite bound_to_free_set_variable_subst with (X := X).
+    5: { apply svar_quantify_not_free. }
+    4: {
          apply svar_quantify_closed_mu.
          unfold well_formed, well_formed_closed in *. destruct_and!. auto.
-      }
-      2: lia.
-      reflexivity.
     }
-
-    2: abstract (wf_auto2).
-
-    eapply (@cast_proof' Σ Γ) in Hpf.
-    2: {
-      rewrite svar_open_svar_quantify.
-      { unfold well_formed, well_formed_closed in *. destruct_and!. auto. }
-      reflexivity.
+    3: {
+         apply svar_quantify_closed_mu.
+         unfold well_formed, well_formed_closed in *. destruct_and!. auto.
     }
+    2: lia.
+    reflexivity.
+  }
 
-
-    assert(well_formed_positive (ϕ₂^[[svar: X ↦ mu , ϕ₂^{{svar: X ↦ 0}}]]) = true).
-    {
-      unfold well_formed, well_formed_closed in *. destruct_and!. simpl; split_and?.
-      apply wfp_free_svar_subst; auto.
-      { apply svar_quantify_closed_mu. auto. }
-      { simpl. split_and!.
-        2: apply well_formed_positive_svar_quantify; assumption.
-        apply no_negative_occurrence_svar_quantify; auto.
-      }
-    }
-
-    assert(well_formed_closed_mu_aux (ϕ₂^[[svar: X ↦ mu , ϕ₂^{{svar: X ↦ 0}}]]) 0 = true).
-    {
-      unfold well_formed, well_formed_closed in *. destruct_and!. simpl; split_and?; auto.
-      replace 0 with (0 + 0) at 3 by lia.
-      apply wfc_mu_free_svar_subst; auto.
-      simpl.
-      apply svar_quantify_closed_mu. assumption.
-    }
-    
-    assert(well_formed_closed_ex_aux (ϕ₂^[[svar: X ↦ mu , ϕ₂^{{svar: X ↦ 0}}]]) 0 = true).
-    {
-      unfold well_formed, well_formed_closed in *. destruct_and!. simpl; split_and?; auto.
-      replace 0 with (0 + 0) at 3 by lia.
-      apply wfc_ex_free_svar_subst; auto.
-      simpl.
-      apply svar_quantify_closed_ex. assumption.
-    }
-
-    assert(well_formed_positive (ϕ₁^[[svar: X ↦ mu , ϕ₂^{{svar: X ↦ 0}}]]) = true).
-    {
-      unfold well_formed, well_formed_closed in *. destruct_and!. simpl; split_and?.
-      apply wfp_free_svar_subst; auto.
-      { apply svar_quantify_closed_mu. auto. }
-      { simpl. split_and!.
-        2: apply well_formed_positive_svar_quantify; assumption.
-        apply no_negative_occurrence_svar_quantify; auto.
-      }
-    }
-
-    assert(well_formed_closed_mu_aux (ϕ₁^[[svar: X ↦ mu , ϕ₂^{{svar: X ↦ 0}}]]) 0 = true).
-    {
-      unfold well_formed, well_formed_closed in *. destruct_and!. simpl; split_and?; auto.
-      replace 0 with (0 + 0) at 3 by lia.
-      apply wfc_mu_free_svar_subst; auto.
-      simpl.
-      apply svar_quantify_closed_mu. assumption.
-    }
-    
-    assert(well_formed_closed_ex_aux (ϕ₁^[[svar: X ↦ mu , ϕ₂^{{svar: X ↦ 0}}]]) 0 = true).
-    {
-      unfold well_formed, well_formed_closed in *. destruct_and!. simpl; split_and?; auto.
-      replace 0 with (0 + 0) at 3 by lia.
-      apply wfc_ex_free_svar_subst; auto.
-      simpl.
-      apply svar_quantify_closed_ex. assumption.
-    }
-
-    apply useBasicReasoning with (i := i) in Hpf.
-    epose proof (Hsi := @syllogism_meta Σ _ _ _ _ _ _ _ _ Htmp Hpf).
-    simpl.
-
-    eapply (@cast_proof' Σ Γ).
-    1: {
-      erewrite bound_to_free_set_variable_subst with (X := X).
-      5: { apply svar_quantify_not_free. }
-      4: {
-           apply svar_quantify_closed_mu.
-           unfold well_formed, well_formed_closed in *. destruct_and!. auto.
-      }
-      3: {
-           apply svar_quantify_closed_mu.
-           unfold well_formed, well_formed_closed in *. destruct_and!. auto.
-      }
-      2: lia.
-      reflexivity.
-    }
-
-    eapply (@cast_proof' Σ Γ).
-    1: {
-      rewrite svar_open_svar_quantify.
-      { unfold well_formed, well_formed_closed in *. destruct_and!. auto. }
-      reflexivity.
-    }
-    apply Hsi.
-    Unshelve.
-    all: abstract(wf_auto2).
-  Defined.
+  eapply (cast_proof' Γ).
+  1: {
+    rewrite svar_open_svar_quantify.
+    { unfold well_formed, well_formed_closed in *. destruct_and!. auto. }
+    reflexivity.
+  }
+  apply Hsi.
+  Unshelve.
+  all: abstract(wf_auto2).
+Defined.
 
 Close Scope ml_scope.
 Close Scope string_scope.
