matching-logic/src/ProofMode_propositional.v
@@ -15,6 +15,7 @@ From MatchingLogic Require Import
     IndexManipulation
     wftactics
     ProofMode_base
+    ProofInfo
 .
 
 From stdpp Require Import list tactics fin_sets coGset gmap sets.
@@ -62,946 +63,946 @@ Arguments P1 {Σ} _ (_%ml) (_%ml) _ _ .
 Arguments P2 {Σ} _ (_%ml) (_%ml) (_%ml) _ _ _.
 Arguments P3 {Σ} _ (_%ml) _.
 
-  Lemma P4m  {Σ : Signature}(Γ : Theory) (A B : Pattern) :
-    well_formed A ->
-    well_formed B ->
-    Γ ⊢i ((A ---> B) ---> ((A ---> !B) ---> !A))
-    using BasicReasoning.
-  Proof.
-    intros WFA WFB.
-    pose (H1 := P2 Γ A B Bot ltac:(wf_auto2) ltac:(wf_auto2) ltac:(wf_auto2)).
-    pose (H2 := (P2 Γ (A ---> B ---> Bot) (A ---> B) (A ---> Bot) ltac:(wf_auto2) ltac:(wf_auto2) ltac:(wf_auto2))).
-    pose (H3 := MP H1 H2).
-    pose (H4 := (P1 Γ (((A ---> B ---> Bot) ---> A ---> B) ---> (A ---> B ---> Bot) ---> A ---> Bot)
-      (A ---> B) ltac:(wf_auto2) ltac:(wf_auto2))).
-    pose (H5 := MP H3 H4).
-    pose (H6 := (P2 Γ (A ---> B) ((A ---> B ---> Bot) ---> A ---> B) ((A ---> B ---> Bot) ---> A ---> Bot)
-      ltac:(wf_auto2) ltac:(wf_auto2) ltac:(wf_auto2))).
-    pose (H7 := MP H5 H6).
-    pose (H8 := (P1 Γ (A ---> B) (A ---> B ---> Bot) ltac:(wf_auto2) ltac:(wf_auto2))).
-    pose (H9 := MP H8 H7).
-    exact H9.
-  Defined.
+Lemma P4m  {Σ : Signature}(Γ : Theory) (A B : Pattern) :
+  well_formed A ->
+  well_formed B ->
+  Γ ⊢i ((A ---> B) ---> ((A ---> !B) ---> !A))
+  using BasicReasoning.
+Proof.
+  intros WFA WFB.
+  pose (H1 := P2 Γ A B Bot ltac:(wf_auto2) ltac:(wf_auto2) ltac:(wf_auto2)).
+  pose (H2 := (P2 Γ (A ---> B ---> Bot) (A ---> B) (A ---> Bot) ltac:(wf_auto2) ltac:(wf_auto2) ltac:(wf_auto2))).
+  pose (H3 := MP H1 H2).
+  pose (H4 := (P1 Γ (((A ---> B ---> Bot) ---> A ---> B) ---> (A ---> B ---> Bot) ---> A ---> Bot)
+    (A ---> B) ltac:(wf_auto2) ltac:(wf_auto2))).
+  pose (H5 := MP H3 H4).
+  pose (H6 := (P2 Γ (A ---> B) ((A ---> B ---> Bot) ---> A ---> B) ((A ---> B ---> Bot) ---> A ---> Bot)
+    ltac:(wf_auto2) ltac:(wf_auto2) ltac:(wf_auto2))).
+  pose (H7 := MP H5 H6).
+  pose (H8 := (P1 Γ (A ---> B) (A ---> B ---> Bot) ltac:(wf_auto2) ltac:(wf_auto2))).
+  pose (H9 := MP H8 H7).
+  exact H9.
+Defined.
 
-  Lemma P4i {Σ : Signature} (Γ : Theory) (A : Pattern) :
-    well_formed A ->
-    Γ ⊢i ((A ---> !A) ---> !A)
-    using BasicReasoning.
-  Proof.
-    intros WFA.
-    eapply MP.
-    { apply (A_impl_A _ A WFA). }
-    { apply (P4m _ A A WFA WFA). }
-  Defined.
+Lemma P4i {Σ : Signature} (Γ : Theory) (A : Pattern) :
+  well_formed A ->
+  Γ ⊢i ((A ---> !A) ---> !A)
+  using BasicReasoning.
+Proof.
+  intros WFA.
+  eapply MP.
+  { apply (A_impl_A _ A WFA). }
+  { apply (P4m _ A A WFA WFA). }
+Defined.
 
-  Lemma reorder {Σ : Signature} (Γ : Theory) (A B C : Pattern) :
-    well_formed A ->
-    well_formed B ->
-    well_formed C ->
-    Γ ⊢i ((A ---> B ---> C) ---> ( B ---> A ---> C))
-    using BasicReasoning.
-  Proof.
-    intros WFA WFB WFC.
+Lemma reorder {Σ : Signature} (Γ : Theory) (A B C : Pattern) :
+  well_formed A ->
+  well_formed B ->
+  well_formed C ->
+  Γ ⊢i ((A ---> B ---> C) ---> ( B ---> A ---> C))
+  using BasicReasoning.
+Proof.
+  intros WFA WFB WFC.
 
-    pose (t1 := (MP
-                    (P1 Γ ((A ---> B) ---> A ---> C) B ltac:(wf_auto2) ltac:(wf_auto2))
-                    (P1 Γ (((A ---> B) ---> A ---> C) ---> B ---> (A ---> B) ---> A ---> C) (A ---> B ---> C) ltac:(wf_auto2) ltac:(wf_auto2)))).
+  pose (t1 := (MP
+                  (P1 Γ ((A ---> B) ---> A ---> C) B ltac:(wf_auto2) ltac:(wf_auto2))
+                  (P1 Γ (((A ---> B) ---> A ---> C) ---> B ---> (A ---> B) ---> A ---> C) (A ---> B ---> C) ltac:(wf_auto2) ltac:(wf_auto2)))).
 
-    pose(ABC := (A ---> B ---> C)).
+  pose(ABC := (A ---> B ---> C)).
 
-    eapply MP.
-    - eapply MP.
-      + apply(P1 _ B A ltac:(wf_auto2) ltac:(wf_auto2)).
-      + apply(P1 _ (B ---> A ---> B) (A ---> B ---> C) ltac:(wf_auto2) ltac:(wf_auto2)).
-    - eapply MP.
-      + eapply MP.
-        * eapply MP.
-          -- eapply MP.
-             ++ apply (A_impl_A _ ABC ltac:(wf_auto2)).
-             ++ eapply MP.
-                ** eapply MP.
-                   --- apply(P2 _ A B C ltac:(wf_auto2) ltac:(wf_auto2) ltac:(wf_auto2)).
-                   --- unshelve (eapply(P1 _ _ (A ---> B ---> C) _ _)); wf_auto2.
-                ** apply P2; wf_auto2.
-          -- eapply MP.
-             ++ apply t1.
-             ++ apply(P2 _ ABC ((A ---> B) ---> (A ---> C)) (B ---> (A ---> B) ---> (A ---> C)) ltac:(wf_auto2) ltac:(wf_auto2) ltac:(wf_auto2)).
-        * eapply MP.
-          -- eapply MP.
-             ++ apply(P2 _ B (A ---> B) (A ---> C) ltac:(wf_auto2) ltac:(wf_auto2) ltac:(wf_auto2)).
-             ++ apply(P1 _ _ ABC); wf_auto2.
-          -- apply P2; wf_auto2.
-      + apply P2; wf_auto2.
-  Defined.
+  eapply MP.
+  - eapply MP.
+    + apply(P1 _ B A ltac:(wf_auto2) ltac:(wf_auto2)).
+    + apply(P1 _ (B ---> A ---> B) (A ---> B ---> C) ltac:(wf_auto2) ltac:(wf_auto2)).
+  - eapply MP.
+    + eapply MP.
+      * eapply MP.
+        -- eapply MP.
+           ++ apply (A_impl_A _ ABC ltac:(wf_auto2)).
+           ++ eapply MP.
+              ** eapply MP.
+                 --- apply(P2 _ A B C ltac:(wf_auto2) ltac:(wf_auto2) ltac:(wf_auto2)).
+                 --- unshelve (eapply(P1 _ _ (A ---> B ---> C) _ _)); wf_auto2.
+              ** apply P2; wf_auto2.
+        -- eapply MP.
+           ++ apply t1.
+           ++ apply(P2 _ ABC ((A ---> B) ---> (A ---> C)) (B ---> (A ---> B) ---> (A ---> C)) ltac:(wf_auto2) ltac:(wf_auto2) ltac:(wf_auto2)).
+      * eapply MP.
+        -- eapply MP.
+           ++ apply(P2 _ B (A ---> B) (A ---> C) ltac:(wf_auto2) ltac:(wf_auto2) ltac:(wf_auto2)).
+           ++ apply(P1 _ _ ABC); wf_auto2.
+        -- apply P2; wf_auto2.
+    + apply P2; wf_auto2.
+Defined.
 
 
-  Lemma reorder_meta {Σ : Signature} {Γ : Theory} {A B C : Pattern} {i : ProofInfo} :
-    well_formed A ->
-    well_formed B ->
-    well_formed C ->  
-    Γ ⊢i (A ---> B ---> C) using i ->
-    Γ ⊢i (B ---> A ---> C) using i.
-  Proof.
-    intros H H0 H1 H2.
-    eapply MP. apply H2.
-    apply useBasicReasoning.
-    apply reorder; wf_auto2.
-  Defined.
+Lemma reorder_meta {Σ : Signature} {Γ : Theory} {A B C : Pattern} {i : ProofInfo} :
+  well_formed A ->
+  well_formed B ->
+  well_formed C ->  
+  Γ ⊢i (A ---> B ---> C) using i ->
+  Γ ⊢i (B ---> A ---> C) using i.
+Proof.
+  intros H H0 H1 H2.
+  eapply MP. apply H2.
+  apply useBasicReasoning.
+  apply reorder; wf_auto2.
+Defined.
 
-  Lemma syllogism {Σ : Signature} (Γ : Theory) (A B C : Pattern) :
-    well_formed A ->
-    well_formed B ->
-    well_formed C ->
-    Γ ⊢i ((A ---> B) ---> (B ---> C) ---> (A ---> C))
-    using BasicReasoning.
-  Proof.
-    intros WFA WFB WFC.
-    apply reorder_meta;[wf_auto2|wf_auto2|wf_auto2|].
-    eapply MP.
-    - apply(P1 _ (B ---> C) A); wf_auto2.
-    - eapply MP.
-      + eapply MP.
-        * apply (P2 _ A B C); wf_auto2.
-        * apply (P1 _ ((A ---> B ---> C) ---> (A ---> B) ---> A ---> C) (B ---> C)); wf_auto2.
-      + apply P2; wf_auto2.
-  Defined.
+Lemma syllogism {Σ : Signature} (Γ : Theory) (A B C : Pattern) :
+  well_formed A ->
+  well_formed B ->
+  well_formed C ->
+  Γ ⊢i ((A ---> B) ---> (B ---> C) ---> (A ---> C))
+  using BasicReasoning.
+Proof.
+  intros WFA WFB WFC.
+  apply reorder_meta;[wf_auto2|wf_auto2|wf_auto2|].
+  eapply MP.
+  - apply(P1 _ (B ---> C) A); wf_auto2.
+  - eapply MP.
+    + eapply MP.
+      * apply (P2 _ A B C); wf_auto2.
+      * apply (P1 _ ((A ---> B ---> C) ---> (A ---> B) ---> A ---> C) (B ---> C)); wf_auto2.
+    + apply P2; wf_auto2.
+Defined.
+
+Lemma syllogism_meta {Σ : Signature} {Γ : Theory} {A B C : Pattern} {i : ProofInfo} :
+  well_formed A ->
+  well_formed B ->
+  well_formed C ->
+  Γ ⊢i (A ---> B) using i ->
+  Γ ⊢i (B ---> C) using i ->
+  Γ ⊢i (A ---> C) using i.
+Proof.
+  intros H H0 H1 H2 H3.
+  eapply MP.
+  - exact H2.
+  - eapply MP.
+    + exact H3.
+    + apply reorder_meta;[wf_auto2|wf_auto2|wf_auto2|].
+      apply useBasicReasoning.
+      apply syllogism; wf_auto2.
+Defined.
+
+Lemma modus_ponens {Σ : Signature} (Γ : Theory) (A B : Pattern) :
+  well_formed A ->
+  well_formed B ->
+  Γ ⊢i (A ---> (A ---> B) ---> B)
+  using BasicReasoning.
+Proof.
+  intros WFA WFB.
+  eapply MP.
+  - apply (P1 _ A (A ---> B) ltac:(wf_auto2) ltac:(wf_auto2)).
+  - eapply MP.
+    + eapply MP.
+      * apply (A_impl_A _ (A ---> B) ltac:(wf_auto2)).
+      * eapply (P2 _ (A ---> B) A B ltac:(wf_auto2) ltac:(wf_auto2) ltac:(wf_auto2)).
+    + apply reorder_meta;[wf_auto2|wf_auto2|wf_auto2|].
+      apply syllogism; wf_auto2.
+Defined.
+
+Lemma not_not_intro {Σ : Signature} (Γ : Theory) (A : Pattern) :
+  well_formed A ->
+  Γ ⊢i (A ---> !(!A))
+  using BasicReasoning.
+Proof.
+  intros WFA.
+  apply modus_ponens; wf_auto2.
+Defined.
+
+Lemma P4 {Σ : Signature} (Γ : Theory) (A B : Pattern)  :
+  well_formed A ->
+  well_formed B -> 
+  Γ ⊢i (((! A) ---> (! B)) ---> (B ---> A))
+  using BasicReasoning.
+Proof.
+  intros WFA WFB.
+  pose proof (m := P3 Γ A ltac:(wf_auto2)).
+  pose proof (m0 := P1 Γ (((A ---> Bot) ---> Bot) ---> A) B ltac:(wf_auto2) ltac:(wf_auto2)).
+  pose proof (m1 := P2 Γ B ((A ---> Bot) ---> Bot) A ltac:(wf_auto2) ltac:(wf_auto2) ltac:(wf_auto2)).
+  pose proof (m2 := MP m m0).
+  pose proof (m3 := MP m2 m1).
+  pose proof (m4 := P1 Γ ((B ---> (A ---> Bot) ---> Bot) ---> B ---> A) ((A ---> Bot) ---> (B ---> Bot)) ltac:(wf_auto2) ltac:(wf_auto2) ).
+  pose proof (m5 := MP m3 m4).
+  pose proof (m6 := P2 Γ ((A ---> Bot) ---> (B ---> Bot)) (B ---> (A ---> Bot) ---> Bot) (B ---> A) ltac:(wf_auto2) ltac:(wf_auto2) ltac:(wf_auto2)).
+  pose proof (m7 := MP m5 m6).
+  pose proof (m8 := reorder Γ (A ---> Bot) (B) Bot ltac:(wf_auto2) ltac:(wf_auto2) ltac:(wf_auto2)).
+  apply (MP m8 m7).
+Defined.
+
+Lemma conj_intro {Σ : Signature} (Γ : Theory) (A B : Pattern) :
+  well_formed A ->
+  well_formed B ->
+  Γ ⊢i (A ---> B ---> (A and B))
+  using BasicReasoning.
+Proof.
+  intros WFA WFB.
+  pose proof (tB := (A_impl_A Γ B ltac:(wf_auto2))).
+  epose proof (t1 := MP (P2 _ (!(!A) ---> !B) A Bot ltac:(wf_auto2) ltac:(wf_auto2) ltac:(wf_auto2)) (P1 _ _ B _ _)).
+  epose proof (t2 := MP (reorder_meta _ _ _ (P4 _ (!A) B ltac:(wf_auto2) ltac:(wf_auto2))) (P1 _ _ B _ _)).
+  epose proof (t3'' := MP (P1 _ A (!(!A) ---> !B) _ _) (P1 _ _ B _ _)).
+  epose proof (t4 := MP tB (MP t2 (P2 _ B B _ _ _ _))).
+  epose proof (t5'' := 
+          MP t4
+                       (MP t1
+                                     (P2 _ B ((!(!A) ---> !B) ---> !A)
+                                         (((!(!A) ---> !B) ---> A) ---> !(!(!A) ---> !B)) _ _ _))).
   
-  Lemma syllogism_meta {Σ : Signature} {Γ : Theory} {A B C : Pattern} {i : ProofInfo} :
-    well_formed A ->
-    well_formed B ->
-    well_formed C ->
-    Γ ⊢i (A ---> B) using i ->
-    Γ ⊢i (B ---> C) using i ->
-    Γ ⊢i (A ---> C) using i.
-  Proof.
-    intros H H0 H1 H2 H3.
-    eapply MP.
-    - exact H2.
-    - eapply MP.
-      + exact H3.
-      + apply reorder_meta;[wf_auto2|wf_auto2|wf_auto2|].
-        apply useBasicReasoning.
-        apply syllogism; wf_auto2.
-  Defined.
+  epose proof (tA := (P1 Γ A B) _ _).
+  epose proof (tB' := MP tB
+                            (P1 _ (B ---> B) A _ _)).
+  epose proof (t3' := MP t3''
+                            (P2 _ B A ((!(!A) ---> !B) ---> A) _ _ _)).
+  epose proof (t3 := MP t3'
+                           (P1 _ ((B ---> A) ---> B ---> (! (! A) ---> ! B) ---> A) A _ _)).
+  epose proof (t5' := MP t5''
+                            (P2 _ B ((!(!A) ---> !B) ---> A) (!(!(!A) ---> !B)) _ _ _)).
+  epose proof (t5 := MP t5' 
+                           (P1 _ ((B ---> (! (! A) ---> ! B) ---> A) ---> B ---> ! (! (! A) ---> ! B))
+                               A _ _)).
+  epose proof (t6 := MP tA
+                           (MP t3
+                                         (P2 _ A (B ---> A) (B ---> (!(!A) ---> !B) ---> A) _ _ _))).
+  epose proof (t7 := MP t6 
+                           (MP t5 
+                                         (P2 _ A (B ---> (!(!A) ---> !B) ---> A) (B ---> !(!(!A) ---> !B)) _ _ _))).
+  apply t7.
+  Unshelve.
+  all: wf_auto2.
+Defined.
 
-  Lemma modus_ponens {Σ : Signature} (Γ : Theory) (A B : Pattern) :
-    well_formed A ->
-    well_formed B ->
-    Γ ⊢i (A ---> (A ---> B) ---> B)
-    using BasicReasoning.
-  Proof.
-    intros WFA WFB.
-    eapply MP.
-    - apply (P1 _ A (A ---> B) ltac:(wf_auto2) ltac:(wf_auto2)).
-    - eapply MP.
-      + eapply MP.
-        * apply (A_impl_A _ (A ---> B) ltac:(wf_auto2)).
-        * eapply (P2 _ (A ---> B) A B ltac:(wf_auto2) ltac:(wf_auto2) ltac:(wf_auto2)).
-      + apply reorder_meta;[wf_auto2|wf_auto2|wf_auto2|].
-        apply syllogism; wf_auto2.
-  Defined.
+Lemma conj_intro_meta {Σ : Signature} (Γ : Theory) (A B : Pattern) (i : ProofInfo) :
+  well_formed A ->
+  well_formed B ->
+  Γ ⊢i A using i ->
+  Γ ⊢i B using i ->
+  Γ ⊢i (A and B) using i.
+Proof.
+  intros WFA WFB H H0.
+  eapply MP.
+  - exact H0.
+  - eapply MP.
+    + exact H.
+    + apply useBasicReasoning.
+      apply conj_intro; wf_auto2.
+Defined.
 
-  Lemma not_not_intro {Σ : Signature} (Γ : Theory) (A : Pattern) :
-    well_formed A ->
-    Γ ⊢i (A ---> !(!A))
-    using BasicReasoning.
-  Proof.
-    intros WFA.
-    apply modus_ponens; wf_auto2.
-  Defined.
+Lemma syllogism_4_meta {Σ : Signature} (Γ : Theory) (A B C D : Pattern) (i : ProofInfo) :
+  well_formed A ->
+  well_formed B ->
+  well_formed C ->
+  well_formed D ->
+  Γ ⊢i (A ---> B ---> C) using i ->
+  Γ ⊢i (C ---> D) using i ->
+  Γ ⊢i (A ---> B ---> D) using i.
+Proof.
+  intros WFA WFB WFC WFD H H0.
+  eapply MP.
+  - exact H.
+  - eapply MP.
+    + eapply MP.
+      * eapply MP.
+        -- eapply MP.
+           ++ exact H0.
+           ++ apply useBasicReasoning. 
+              eapply (P1 _ (C ---> D) B _ _).
+        -- apply useBasicReasoning.  
+            eapply (P2 _ B C D _ _ _).
+      * apply useBasicReasoning. 
+        eapply (P1 _ ((B ---> C) ---> B ---> D) A _ _).
+    + apply useBasicReasoning. 
+      eapply (P2 _ A (B ---> C) (B ---> D) _ _ _).
+      Unshelve.
+      all: wf_auto2.
+Defined.
 
-  Lemma P4 {Σ : Signature} (Γ : Theory) (A B : Pattern)  :
-    well_formed A ->
-    well_formed B -> 
-    Γ ⊢i (((! A) ---> (! B)) ---> (B ---> A))
-    using BasicReasoning.
-  Proof.
-    intros WFA WFB.
-    pose proof (m := P3 Γ A ltac:(wf_auto2)).
-    pose proof (m0 := P1 Γ (((A ---> Bot) ---> Bot) ---> A) B ltac:(wf_auto2) ltac:(wf_auto2)).
-    pose proof (m1 := P2 Γ B ((A ---> Bot) ---> Bot) A ltac:(wf_auto2) ltac:(wf_auto2) ltac:(wf_auto2)).
-    pose proof (m2 := MP m m0).
-    pose proof (m3 := MP m2 m1).
-    pose proof (m4 := P1 Γ ((B ---> (A ---> Bot) ---> Bot) ---> B ---> A) ((A ---> Bot) ---> (B ---> Bot)) ltac:(wf_auto2) ltac:(wf_auto2) ).
-    pose proof (m5 := MP m3 m4).
-    pose proof (m6 := P2 Γ ((A ---> Bot) ---> (B ---> Bot)) (B ---> (A ---> Bot) ---> Bot) (B ---> A) ltac:(wf_auto2) ltac:(wf_auto2) ltac:(wf_auto2)).
-    pose proof (m7 := MP m5 m6).
-    pose proof (m8 := reorder Γ (A ---> Bot) (B) Bot ltac:(wf_auto2) ltac:(wf_auto2) ltac:(wf_auto2)).
-    apply (MP m8 m7).
-  Defined.
-
-  Lemma conj_intro {Σ : Signature} (Γ : Theory) (A B : Pattern) :
-    well_formed A ->
-    well_formed B ->
-    Γ ⊢i (A ---> B ---> (A and B))
-    using BasicReasoning.
-  Proof.
-    intros WFA WFB.
-    pose proof (tB := (A_impl_A Γ B ltac:(wf_auto2))).
-    epose proof (t1 := MP (P2 _ (!(!A) ---> !B) A Bot ltac:(wf_auto2) ltac:(wf_auto2) ltac:(wf_auto2)) (P1 _ _ B _ _)).
-    epose proof (t2 := MP (reorder_meta _ _ _ (P4 _ (!A) B ltac:(wf_auto2) ltac:(wf_auto2))) (P1 _ _ B _ _)).
-    epose proof (t3'' := MP (P1 _ A (!(!A) ---> !B) _ _) (P1 _ _ B _ _)).
-    epose proof (t4 := MP tB (MP t2 (P2 _ B B _ _ _ _))).
-    epose proof (t5'' := 
-            MP t4
-                         (MP t1
-                                       (P2 _ B ((!(!A) ---> !B) ---> !A)
-                                           (((!(!A) ---> !B) ---> A) ---> !(!(!A) ---> !B)) _ _ _))).
-    
-    epose proof (tA := (P1 Γ A B) _ _).
-    epose proof (tB' := MP tB
-                              (P1 _ (B ---> B) A _ _)).
-    epose proof (t3' := MP t3''
-                              (P2 _ B A ((!(!A) ---> !B) ---> A) _ _ _)).
-    epose proof (t3 := MP t3'
-                             (P1 _ ((B ---> A) ---> B ---> (! (! A) ---> ! B) ---> A) A _ _)).
-    epose proof (t5' := MP t5''
-                              (P2 _ B ((!(!A) ---> !B) ---> A) (!(!(!A) ---> !B)) _ _ _)).
-    epose proof (t5 := MP t5' 
-                             (P1 _ ((B ---> (! (! A) ---> ! B) ---> A) ---> B ---> ! (! (! A) ---> ! B))
-                                 A _ _)).
-    epose proof (t6 := MP tA
-                             (MP t3
-                                           (P2 _ A (B ---> A) (B ---> (!(!A) ---> !B) ---> A) _ _ _))).
-    epose proof (t7 := MP t6 
-                             (MP t5 
-                                           (P2 _ A (B ---> (!(!A) ---> !B) ---> A) (B ---> !(!(!A) ---> !B)) _ _ _))).
-    apply t7.
+Lemma bot_elim {Σ : Signature} (Γ : Theory) (A : Pattern) :
+  well_formed A ->
+  Γ ⊢i (Bot ---> A)
+  using BasicReasoning.
+Proof.
+  intros WFA.
+  eapply MP.
+  - eapply MP.
+    + eapply MP.
+      * eapply MP.
+        -- eapply (P1 _ Bot Bot _ _).
+        -- eapply (P2 _ Bot Bot Bot _ _ _).
+      * eapply (P4 _ Bot Bot _ _).
+    + eapply (P1 _ (Bot ---> Bot) (A ---> Bot) _ _).
+  - eapply (P4 _ A Bot _ _).
     Unshelve.
     all: wf_auto2.
-  Defined.
+Defined.
 
-  Lemma conj_intro_meta {Σ : Signature} (Γ : Theory) (A B : Pattern) (i : ProofInfo) :
-    well_formed A ->
-    well_formed B ->
-    Γ ⊢i A using i ->
-    Γ ⊢i B using i ->
-    Γ ⊢i (A and B) using i.
-  Proof.
-    intros WFA WFB H H0.
-    eapply MP.
-    - exact H0.
-    - eapply MP.
-      + exact H.
-      + apply useBasicReasoning.
-        apply conj_intro; wf_auto2.
-  Defined.
-  
-  Lemma syllogism_4_meta {Σ : Signature} (Γ : Theory) (A B C D : Pattern) (i : ProofInfo) :
-    well_formed A ->
-    well_formed B ->
-    well_formed C ->
-    well_formed D ->
-    Γ ⊢i (A ---> B ---> C) using i ->
-    Γ ⊢i (C ---> D) using i ->
-    Γ ⊢i (A ---> B ---> D) using i.
-  Proof.
-    intros WFA WFB WFC WFD H H0.
-    eapply MP.
-    - exact H.
-    - eapply MP.
-      + eapply MP.
-        * eapply MP.
-          -- eapply MP.
-             ++ exact H0.
-             ++ apply useBasicReasoning. 
-                eapply (P1 _ (C ---> D) B _ _).
-          -- apply useBasicReasoning.  
-              eapply (P2 _ B C D _ _ _).
-        * apply useBasicReasoning. 
-          eapply (P1 _ ((B ---> C) ---> B ---> D) A _ _).
-      + apply useBasicReasoning. 
-        eapply (P2 _ A (B ---> C) (B ---> D) _ _ _).
-        Unshelve.
-        all: wf_auto2.
-  Defined.
+Lemma modus_ponens' {Σ : Signature} (Γ : Theory) (A B : Pattern) :
+  well_formed A ->
+  well_formed B ->
+  Γ ⊢i (A ---> (!B ---> !A) ---> B)
+  using BasicReasoning.
+Proof.
+  intros WFA WFB.
+  apply reorder_meta;[wf_auto2|wf_auto2|wf_auto2|].
+  apply P4; wf_auto2.
+Defined.
 
-  Lemma bot_elim {Σ : Signature} (Γ : Theory) (A : Pattern) :
-    well_formed A ->
-    Γ ⊢i (Bot ---> A)
-    using BasicReasoning.
-  Proof.
-    intros WFA.
-    eapply MP.
-    - eapply MP.
-      + eapply MP.
-        * eapply MP.
-          -- eapply (P1 _ Bot Bot _ _).
-          -- eapply (P2 _ Bot Bot Bot _ _ _).
-        * eapply (P4 _ Bot Bot _ _).
-      + eapply (P1 _ (Bot ---> Bot) (A ---> Bot) _ _).
-    - eapply (P4 _ A Bot _ _).
-      Unshelve.
-      all: wf_auto2.
-  Defined.
+Lemma disj_right_intro {Σ : Signature} (Γ : Theory) (A B : Pattern) :
+  well_formed A ->
+  well_formed B ->
+  Γ ⊢i (B ---> (A or B))
+  using BasicReasoning.
+Proof.
+  intros WFA WFB.
+  apply useBasicReasoning.
+  apply P1; wf_auto2.
+Defined.
 
-  Lemma modus_ponens' {Σ : Signature} (Γ : Theory) (A B : Pattern) :
-    well_formed A ->
-    well_formed B ->
-    Γ ⊢i (A ---> (!B ---> !A) ---> B)
-    using BasicReasoning.
-  Proof.
-    intros WFA WFB.
-    apply reorder_meta;[wf_auto2|wf_auto2|wf_auto2|].
-    apply P4; wf_auto2.
-  Defined.
+Lemma disj_left_intro {Σ : Signature} (Γ : Theory) (A B : Pattern) :
+  well_formed A ->
+  well_formed B ->
+  Γ ⊢i (A ---> (A or B))
+  using BasicReasoning.
+Proof.
+  intros WFA WFB.
+  eapply syllogism_4_meta.
+  5: { apply modus_ponens; wf_auto2. }
+  5: { apply bot_elim; wf_auto2. }
+  all: wf_auto2.
+Defined.
 
-  Lemma disj_right_intro {Σ : Signature} (Γ : Theory) (A B : Pattern) :
-    well_formed A ->
-    well_formed B ->
-    Γ ⊢i (B ---> (A or B))
-    using BasicReasoning.
-  Proof.
-    intros WFA WFB.
+Lemma disj_right_intro_meta {Σ : Signature} (Γ : Theory) (A B : Pattern) (i : ProofInfo) :
+  well_formed A ->
+  well_formed B ->
+  Γ ⊢i B using i ->
+  Γ ⊢i (A or B) using i.
+Proof.
+  intros HwfA HwfB HB.
+  eapply MP.
+  { exact HB. }
+  {
     apply useBasicReasoning.
+    apply disj_right_intro; wf_auto2.
+  }
+Defined.
+
+Lemma disj_left_intro_meta {Σ : Signature} (Γ : Theory) (A B : Pattern) (i : ProofInfo) :
+  well_formed A ->
+  well_formed B ->
+  Γ ⊢i A using i ->
+  Γ ⊢i (A or B) using i.
+Proof.
+  intros HwfA HwfB HA.
+  eapply MP.
+  { exact HA. }
+  apply useBasicReasoning.
+  apply disj_left_intro; assumption.
+Defined.
+
+Lemma not_not_elim {Σ : Signature} (Γ : Theory) (A : Pattern) :
+  well_formed A ->
+  Γ ⊢i (!(!A) ---> A)
+  using BasicReasoning.
+Proof.
+  intros WFA.
+  apply P3. exact WFA.
+Defined.
+
+Lemma not_not_elim_meta {Σ : Signature} Γ A (i : ProofInfo) :
+  well_formed A ->
+  Γ ⊢i (! ! A) using i ->
+  Γ ⊢i A using i.
+Proof.
+  intros wfA nnA.
+  eapply MP.
+  { apply nnA. }
+  { apply useBasicReasoning. apply not_not_elim. exact wfA. }
+Defined.
+
+Lemma double_neg_elim {Σ : Signature} (Γ : Theory) (A B : Pattern) :
+  well_formed A ->
+  well_formed B ->
+  Γ ⊢i (((!(!A)) ---> (!(!B))) ---> (A ---> B))
+  using BasicReasoning.
+Proof.
+  intros WFA WFB.
+  eapply syllogism_meta.
+  5: apply P4.
+  4: apply P4.
+  all: wf_auto2.
+Defined.
+
+Lemma double_neg_elim_meta {Σ : Signature} (Γ : Theory) (A B : Pattern) (i : ProofInfo) :
+  well_formed A ->
+  well_formed B -> 
+  Γ ⊢i ((!(!A)) ---> (!(!B))) using i ->
+  Γ ⊢i (A ---> B) using i.
+Proof.
+  intros WFA WFB H.
+  eapply MP.
+  - exact H.
+  - apply useBasicReasoning.
+    apply double_neg_elim; wf_auto2.
+Defined.
+
+Lemma not_not_impl_intro {Σ : Signature} (Γ : Theory) (A B : Pattern) :
+  well_formed A ->
+  well_formed B ->
+  Γ ⊢i ((A ---> B) ---> ((! ! A) ---> (! ! B)))
+  using BasicReasoning.
+Proof.
+  intros WFA WFB.
+
+  epose (S1 := syllogism Γ (! ! A) A B _ _ _).
+
+  epose (MP1 := MP (not_not_elim _ A _) S1).
+
+  epose(NNB := not_not_intro Γ B _).
+
+  epose(P1 := (P1 Γ (B ---> ! (! B)) (! ! A) _ _)).
+
+  epose(MP2 := MP NNB P1).
+
+  epose(P2' := (P2 Γ (! ! A) B (! !B) _ _ _)).
+
+  epose(MP3 := MP MP2 P2').
+
+  eapply @syllogism_meta with (B := (! (! A) ---> B)).
+  - shelve.
+  - shelve.
+  - shelve.
+  - assumption.
+  - assumption.
+    Unshelve.
+    all: wf_auto2.
+Defined.
+
+Lemma contraposition {Σ : Signature} (Γ : Theory) (A B : Pattern) : 
+  well_formed A ->
+  well_formed B -> 
+  Γ ⊢i ((A ---> B) ---> ((! B) ---> (! A)))
+  using BasicReasoning.
+Proof.
+  intros WFA WFB.
+  epose proof (P4 Γ (! A) (! B) _ _) as m.
+  apply @syllogism_meta with (B := (! (! A) ---> ! (! B))).
+  - shelve.
+  - shelve.
+  - shelve.
+  - apply not_not_impl_intro; wf_auto2.
+  - exact m. (* apply (P4 _ _ _). shelve. shelve. *)
+    Unshelve.
+    all: wf_auto2.
+Defined.
+
+Lemma or_comm_meta {Σ : Signature} (Γ : Theory) (A B : Pattern) (i : ProofInfo):
+  well_formed A ->
+  well_formed B ->
+  Γ ⊢i (A or B) using i ->
+  Γ ⊢i (B or A) using i.
+Proof.
+  intros WFA WFB H. unfold patt_or in *.
+  epose proof (P4 := (P4 Γ A (!B) _ _)).
+  epose proof (NNI := not_not_intro  Γ B _).
+  apply (useBasicReasoning i) in P4.
+  apply (useBasicReasoning i) in NNI.
+  epose proof (SI := syllogism_meta _ _ _ H NNI).
+  eapply MP.
+  - exact SI.
+  - exact P4.
+    Unshelve.
+    all: wf_auto2.
+Defined.
+
+Lemma A_implies_not_not_A_alt {Σ : Signature} (Γ : Theory) (A : Pattern) (i : ProofInfo) :
+  well_formed A ->
+  Γ ⊢i A using i ->
+  Γ ⊢i (!( !A )) using i.
+Proof.
+  intros WFA H. unfold patt_not.
+  eapply MP.
+  { apply H. }
+  {
+    apply useBasicReasoning.
+    apply not_not_intro.
+    exact WFA.
+  }
+Defined.
+
+Lemma P5i {Σ : Signature} (Γ : Theory) (A B : Pattern) :
+  well_formed A ->
+  well_formed B ->
+  Γ ⊢i (! A ---> (A ---> B))
+  using BasicReasoning.
+Proof.
+  intros WFA WFB.
+  eapply syllogism_meta.
+  5: apply P4.
+  4: apply P1.
+  all: wf_auto2.
+Defined.
+
+Lemma A_implies_not_not_A_alt_Γ {Σ : Signature} (Γ : Theory) (A : Pattern) (i : ProofInfo) :
+  well_formed A ->
+  Γ ⊢i A using i ->
+  Γ ⊢i (!( !A )) using i.
+Proof.
+  intros WFA H. unfold patt_not.
+  eapply MP.
+  { apply H. }
+  { apply useBasicReasoning. apply not_not_intro. exact WFA. }
+Defined.
+
+
+Lemma exclusion {Σ : Signature} (G : Theory) (A : Pattern) (i : ProofInfo) :
+  well_formed A ->
+  G ⊢i A using i ->
+  G ⊢i (A ---> Bot) using i ->
+  G ⊢i Bot using i.
+Proof.
+  intros WFA H H0.
+  eapply MP.
+  apply H.
+  apply H0.
+Defined.
+
+Lemma modus_tollens {Σ : Signature} Γ A B (i : ProofInfo) :
+  Γ ⊢i (A ---> B) using i ->
+  Γ ⊢i (!B ---> !A) using i.
+Proof.
+  intros H.
+  pose proof (wf := proved_impl_wf _ _ (proj1_sig H)).
+  assert (wfA : well_formed A) by wf_auto2.
+  assert (wfB : well_formed B) by wf_auto2.
+
+  eapply MP.
+  2: { apply useBasicReasoning. apply contraposition; wf_auto2. }
+  apply H.
+Defined.
+
+Lemma A_impl_not_not_B {Σ : Signature} Γ A B :
+  well_formed A ->
+  well_formed B ->
+  Γ ⊢i ((A ---> ! !B) ---> (A ---> B))
+  using BasicReasoning.
+Proof.
+  intros WFA WFB.
+
+  assert (H0 : Γ ⊢i (! !B ---> B) using BasicReasoning).
+  {
+    apply not_not_elim. wf_auto2.
+  }
+
+  assert (H1 : Γ ⊢i ((A ---> ! !B) ---> (! !B ---> B) ---> (A ---> B)) using BasicReasoning).
+  {
+    apply syllogism; wf_auto2.
+  }
+
+  eapply MP.
+  2: { 
+    apply reorder_meta.
+    4: apply H1.
+    all: wf_auto2.
+  }
+  apply H0.
+Defined.
+
+Lemma prf_weaken_conclusion {Σ : Signature} Γ A B B' :
+  well_formed A ->
+  well_formed B ->
+  well_formed B' ->
+  Γ ⊢i ((B ---> B') ---> ((A ---> B) ---> (A ---> B')))
+  using BasicReasoning.
+Proof.
+  intros wfA wfB wfB'.
+  apply reorder_meta;[wf_auto2|wf_auto2|wf_auto2|].
+  apply syllogism; wf_auto2.
+Defined.
+
+Lemma prf_weaken_conclusion_meta {Σ : Signature} Γ A B B' (i : ProofInfo) :
+  well_formed A ->
+  well_formed B ->
+  well_formed B' ->
+  Γ ⊢i (B ---> B') using i ->
+  Γ ⊢i ((A ---> B) ---> (A ---> B')) using i.
+Proof.
+  intros wfA wfB wfB' BimpB'.
+  assert (H1: Γ ⊢i ((A ---> B) ---> (B ---> B') ---> (A ---> B')) using i).
+  {
+    apply useBasicReasoning. apply syllogism; wf_auto2.
+  }
+  apply reorder_meta in H1;[|wf_auto2|wf_auto2|wf_auto2].
+  eapply MP. 2: apply H1. apply BimpB'.
+Defined.
+
+Lemma prf_weaken_conclusion_iter {Σ : Signature} Γ l g g'
+        (wfl : Pattern.wf l) (wfg : well_formed g) (wfg' : well_formed g') :
+  Γ ⊢i ((g ---> g') ---> (fold_right patt_imp g l ---> fold_right patt_imp g' l))
+  using BasicReasoning.
+Proof.
+  induction l.
+  - apply A_impl_A. wf_auto2.
+  - pose proof (wfl' := wfl).
+    apply andb_prop in wfl.
+    fold (map well_formed) in wfl.
+    destruct wfl as [wfa wfl].
+    (* fold does not work in wfl, so I just assert & clear. *)
+    assert (wfl'' : Pattern.wf l) by apply wfl.
+    clear wfl.
+    specialize (IHl wfl'').
+    simpl in *.
+    eapply syllogism_meta.
+    5: eapply prf_weaken_conclusion.
+    4: apply IHl.
+    all: wf_auto2.
+Defined.
+
+Lemma prf_weaken_conclusion_iter_meta {Σ : Signature} Γ l g g' (i : ProofInfo):
+  Pattern.wf l ->
+  well_formed g ->
+  well_formed g' ->
+  Γ ⊢i (g ---> g') using i ->
+  Γ ⊢i ((fold_right patt_imp g l) ---> (fold_right patt_imp g' l)) using i.
+Proof.
+  intros wfl wfg wfg' gimpg'.
+  eapply MP.
+  2: { apply useBasicReasoning. apply prf_weaken_conclusion_iter; wf_auto2. }
+  1: { apply gimpg'. }
+Defined.
+
+Lemma prf_weaken_conclusion_iter_meta_meta {Σ : Signature} Γ l g g' (i : ProofInfo):
+  Pattern.wf l ->
+  well_formed g ->
+  well_formed g' ->
+  Γ ⊢i (g ---> g') using i ->
+  Γ ⊢i (fold_right patt_imp g l) using i ->
+  Γ ⊢i (fold_right patt_imp g' l) using i.
+Proof.
+  intros wfl wfg wfg' gimpg' H.
+  eapply MP.
+  { apply gimpg'. }
+  eapply MP.
+  { apply H. }
+  apply reorder_meta;[wf_auto2|wf_auto2|wf_auto2|].
+  apply useBasicReasoning.
+  apply prf_weaken_conclusion_iter.
+  all: wf_auto2.
+Defined.
+
+Lemma prf_weaken_conclusion_meta_meta {Σ : Signature} Γ A B B' (i : ProofInfo) :
+  well_formed A ->
+  well_formed B ->
+  well_formed B' ->
+  Γ ⊢i (B ---> B') using i ->
+  Γ ⊢i (A ---> B) using i ->
+  Γ ⊢i (A ---> B') using i.
+Proof.
+  intros WFA WFB WFB' H H0.
+  eapply MP. 2: apply prf_weaken_conclusion_meta. 1: apply H0.
+  4: apply H. all: wf_auto2.
+Defined.
+
+Lemma prf_strenghten_premise {Σ : Signature} Γ A A' B :
+  well_formed A ->
+  well_formed A' ->
+  well_formed B ->
+  Γ ⊢i ((A' ---> A) ---> ((A ---> B) ---> (A' ---> B))) using BasicReasoning.
+Proof.
+  intros wfA wfA' wfB.
+  apply syllogism; wf_auto2.
+Defined.
+
+Lemma prf_strenghten_premise_iter {Σ : Signature}  Γ l₁ l₂ h h' g :
+  Pattern.wf l₁ -> Pattern.wf l₂ ->
+  well_formed h ->
+  well_formed h' ->
+  well_formed g ->
+  Γ ⊢i (h' ---> h) --->
+      foldr patt_imp g (l₁ ++ h::l₂) --->
+      foldr patt_imp g (l₁ ++ h'::l₂)
+  using BasicReasoning.
+Proof.
+  intros wfl₁ wfl₂ wfh wfh' wfg.
+  induction l₁.
+  - simpl. apply prf_strenghten_premise. all: wf_auto2.
+  - pose proof (wfal₁ := wfl₁).
+    remember (foldr patt_imp g (h::l₂)) as g1.
+    remember (foldr patt_imp g (h'::l₂)) as g2.
+    unfold Pattern.wf in wfl₁. simpl in wfl₁. apply andb_prop in wfl₁.
+    destruct wfl₁ as [wfa wfl₁].
+    specialize (IHl₁ wfl₁).
+    remember (foldr patt_imp g (l₁ ++ h::l₂)) as b.
+    remember (foldr patt_imp g (l₁ ++ h'::l₂)) as b'.
+
+    assert (prf: Γ ⊢i ((b ---> b') ---> ((a ---> b) ---> (a ---> b'))) using BasicReasoning).
+    { apply prf_weaken_conclusion; subst; wf_auto2. }
+
+    subst.
+    eapply syllogism_meta.
+    5: { apply prf. }
+    4: { apply IHl₁. }
+    all: wf_auto2.
+Defined.
+
+Lemma prf_strenghten_premise_meta {Σ : Signature} Γ A A' B (i : ProofInfo) :
+  well_formed A ->
+  well_formed A' ->
+  well_formed B ->
+  Γ ⊢i (A' ---> A) using i ->
+  Γ ⊢i ((A ---> B) ---> (A' ---> B)) using i.
+Proof.
+  intros wfA wfA' wfB A'impA.
+  assert (H1: Γ ⊢i ((A' ---> A) ---> (A ---> B) ---> (A' ---> B)) using i).
+  {
+    apply useBasicReasoning. apply syllogism; wf_auto2.
+  }
+  eapply MP. 2: apply H1. apply A'impA.
+Defined.
+
+Lemma prf_strenghten_premise_meta_meta {Σ : Signature} Γ A A' B (i : ProofInfo) :
+  well_formed A ->
+  well_formed A' ->
+  well_formed B ->
+  Γ ⊢i (A' ---> A) using i ->
+  Γ ⊢i (A ---> B) using i ->
+  Γ ⊢i (A' ---> B) using i.
+Proof.
+  intros wfA wfA' wfB A'impA AimpB.
+  eapply MP. 2: apply prf_strenghten_premise_meta. 1: apply AimpB.
+  4: apply A'impA. all: wf_auto2.
+Defined.
+
+Lemma prf_strenghten_premise_iter_meta {Σ : Signature} Γ l₁ l₂ h h' g (i : ProofInfo) :
+  Pattern.wf l₁ -> Pattern.wf l₂ ->
+  well_formed h ->
+  well_formed h' ->
+  well_formed g ->
+  Γ ⊢i (h' ---> h) using i ->
+  Γ ⊢i foldr patt_imp g (l₁ ++ h::l₂) --->
+       foldr patt_imp g (l₁ ++ h'::l₂)
+  using i.
+Proof.
+  intros WFl₁ WFl₂ WFh WFh' WFg H.
+  eapply MP.
+  2: { apply useBasicReasoning. apply prf_strenghten_premise_iter; wf_auto2. }
+  exact H.
+Defined.
+
+Lemma prf_strenghten_premise_iter_meta_meta {Σ : Signature} Γ l₁ l₂ h h' g (i : ProofInfo) :
+  Pattern.wf l₁ -> Pattern.wf l₂ ->
+  well_formed h ->
+  well_formed h' ->
+  well_formed g ->
+  Γ ⊢i (h' ---> h) using i ->
+  Γ ⊢i foldr patt_imp g (l₁ ++ h::l₂) using i ->
+  Γ ⊢i foldr patt_imp g (l₁ ++ h'::l₂) using i.  
+Proof.
+  intros WFl₁ WFl₂ WFh WFh' WFg H H0.
+  eapply MP.
+  2: eapply prf_strenghten_premise_iter_meta.
+  7: eassumption. 1: assumption. all: wf_auto2.
+Defined.
+
+
+Local Example example_nested_const {Σ : Signature} Γ a b c:
+  well_formed a ->
+  well_formed b ->
+  well_formed c ->
+  (* like P2 but nested a bit *)
+  Γ ⊢i (a ---> (b ---> (c ---> a)))
+  using BasicReasoning.
+Proof.
+  intros wfa wfb wfc.
+  assert (H1: Γ ⊢i ((c ---> a) ---> (b ---> (c ---> a))) using BasicReasoning).
+  {
     apply P1; wf_auto2.
-  Defined.
-  
-  Lemma disj_left_intro {Σ : Signature} (Γ : Theory) (A B : Pattern) :
-    well_formed A ->
-    well_formed B ->
-    Γ ⊢i (A ---> (A or B))
-    using BasicReasoning.
-  Proof.
-    intros WFA WFB.
-    eapply syllogism_4_meta.
-    5: { apply modus_ponens; wf_auto2. }
-    5: { apply bot_elim; wf_auto2. }
-    all: wf_auto2.
-  Defined.
+  }
+  assert (H2: Γ ⊢i (a ---> (c ---> a)) using BasicReasoning).
+  { apply P1; wf_auto2. }
 
-  Lemma disj_right_intro_meta {Σ : Signature} (Γ : Theory) (A B : Pattern) (i : ProofInfo) :
-    well_formed A ->
-    well_formed B ->
-    Γ ⊢i B using i ->
-    Γ ⊢i (A or B) using i.
-  Proof.
-    intros HwfA HwfB HB.
-    eapply MP.
-    { exact HB. }
-    {
-      apply useBasicReasoning.
-      apply disj_right_intro; wf_auto2.
-    }
-  Defined.
+  eapply (syllogism_meta _ _ _ H2 H1).
+  Unshelve. all: wf_auto2.
+Defined.
 
-  Lemma disj_left_intro_meta {Σ : Signature} (Γ : Theory) (A B : Pattern) (i : ProofInfo) :
-    well_formed A ->
-    well_formed B ->
-    Γ ⊢i A using i ->
-    Γ ⊢i (A or B) using i.
-  Proof.
-    intros HwfA HwfB HA.
-    eapply MP.
-    { exact HA. }
-    apply useBasicReasoning.
-    apply disj_left_intro; assumption.
-  Defined.
-
-  Lemma not_not_elim {Σ : Signature} (Γ : Theory) (A : Pattern) :
-    well_formed A ->
-    Γ ⊢i (!(!A) ---> A)
-    using BasicReasoning.
-  Proof.
-    intros WFA.
-    apply P3. exact WFA.
-  Defined.
-
-  Lemma not_not_elim_meta {Σ : Signature} Γ A (i : ProofInfo) :
-    well_formed A ->
-    Γ ⊢i (! ! A) using i ->
-    Γ ⊢i A using i.
-  Proof.
-    intros wfA nnA.
-    eapply MP.
-    { apply nnA. }
-    { apply useBasicReasoning. apply not_not_elim. exact wfA. }
-  Defined.
-
-  Lemma double_neg_elim {Σ : Signature} (Γ : Theory) (A B : Pattern) :
-    well_formed A ->
-    well_formed B ->
-    Γ ⊢i (((!(!A)) ---> (!(!B))) ---> (A ---> B))
-    using BasicReasoning.
-  Proof.
-    intros WFA WFB.
-    eapply syllogism_meta.
-    5: apply P4.
-    4: apply P4.
-    all: wf_auto2.
-  Defined.
-
-  Lemma double_neg_elim_meta {Σ : Signature} (Γ : Theory) (A B : Pattern) (i : ProofInfo) :
-    well_formed A ->
-    well_formed B -> 
-    Γ ⊢i ((!(!A)) ---> (!(!B))) using i ->
-    Γ ⊢i (A ---> B) using i.
-  Proof.
-    intros WFA WFB H.
-    eapply MP.
-    - exact H.
-    - apply useBasicReasoning.
-      apply double_neg_elim; wf_auto2.
-  Defined.
-
-  Lemma not_not_impl_intro {Σ : Signature} (Γ : Theory) (A B : Pattern) :
-    well_formed A ->
-    well_formed B ->
-    Γ ⊢i ((A ---> B) ---> ((! ! A) ---> (! ! B)))
-    using BasicReasoning.
-  Proof.
-    intros WFA WFB.
-
-    epose (S1 := syllogism Γ (! ! A) A B _ _ _).
-
-    epose (MP1 := MP (not_not_elim _ A _) S1).
-
-    epose(NNB := not_not_intro Γ B _).
-
-    epose(P1 := (P1 Γ (B ---> ! (! B)) (! ! A) _ _)).
-
-    epose(MP2 := MP NNB P1).
-
-    epose(P2' := (P2 Γ (! ! A) B (! !B) _ _ _)).
-
-    epose(MP3 := MP MP2 P2').
-
-    eapply @syllogism_meta with (B := (! (! A) ---> B)).
-    - shelve.
-    - shelve.
-    - shelve.
-    - assumption.
-    - assumption.
-      Unshelve.
-      all: wf_auto2.
-  Defined.
-
-  Lemma contraposition {Σ : Signature} (Γ : Theory) (A B : Pattern) : 
-    well_formed A ->
-    well_formed B -> 
-    Γ ⊢i ((A ---> B) ---> ((! B) ---> (! A)))
-    using BasicReasoning.
-  Proof.
-    intros WFA WFB.
-    epose proof (P4 Γ (! A) (! B) _ _) as m.
-    apply @syllogism_meta with (B := (! (! A) ---> ! (! B))).
-    - shelve.
-    - shelve.
-    - shelve.
-    - apply not_not_impl_intro; wf_auto2.
-    - exact m. (* apply (P4 _ _ _). shelve. shelve. *)
-      Unshelve.
-      all: wf_auto2.
-  Defined.
-
-  Lemma or_comm_meta {Σ : Signature} (Γ : Theory) (A B : Pattern) (i : ProofInfo):
-    well_formed A ->
-    well_formed B ->
-    Γ ⊢i (A or B) using i ->
-    Γ ⊢i (B or A) using i.
-  Proof.
-    intros WFA WFB H. unfold patt_or in *.
-    epose proof (P4 := (P4 Γ A (!B) _ _)).
-    epose proof (NNI := not_not_intro  Γ B _).
-    apply (useBasicReasoning i) in P4.
-    apply (useBasicReasoning i) in NNI.
-    epose proof (SI := syllogism_meta _ _ _ H NNI).
-    eapply MP.
-    - exact SI.
-    - exact P4.
-      Unshelve.
-      all: wf_auto2.
-  Defined.
-
-  Lemma A_implies_not_not_A_alt {Σ : Signature} (Γ : Theory) (A : Pattern) (i : ProofInfo) :
-    well_formed A ->
-    Γ ⊢i A using i ->
-    Γ ⊢i (!( !A )) using i.
-  Proof.
-    intros WFA H. unfold patt_not.
-    eapply MP.
-    { apply H. }
-    {
-      apply useBasicReasoning.
-      apply not_not_intro.
-      exact WFA.
-    }
-  Defined.
-
-  Lemma P5i {Σ : Signature} (Γ : Theory) (A B : Pattern) :
-    well_formed A ->
-    well_formed B ->
-    Γ ⊢i (! A ---> (A ---> B))
-    using BasicReasoning.
-  Proof.
-    intros WFA WFB.
-    eapply syllogism_meta.
-    5: apply P4.
-    4: apply P1.
-    all: wf_auto2.
-  Defined.
-
-  Lemma A_implies_not_not_A_alt_Γ {Σ : Signature} (Γ : Theory) (A : Pattern) (i : ProofInfo) :
-    well_formed A ->
-    Γ ⊢i A using i ->
-    Γ ⊢i (!( !A )) using i.
-  Proof.
-    intros WFA H. unfold patt_not.
-    eapply MP.
-    { apply H. }
-    { apply useBasicReasoning. apply not_not_intro. exact WFA. }
-  Defined.
-
-
-  Lemma exclusion {Σ : Signature} (G : Theory) (A : Pattern) (i : ProofInfo) :
-    well_formed A ->
-    G ⊢i A using i ->
-    G ⊢i (A ---> Bot) using i ->
-    G ⊢i Bot using i.
-  Proof.
-    intros WFA H H0.
-    eapply MP.
-    apply H.
-    apply H0.
-  Defined.
-
-  Lemma modus_tollens {Σ : Signature} Γ A B (i : ProofInfo) :
-    Γ ⊢i (A ---> B) using i ->
-    Γ ⊢i (!B ---> !A) using i.
-  Proof.
-    intros H.
-    pose proof (wf := proved_impl_wf _ _ (proj1_sig H)).
-    assert (wfA : well_formed A) by wf_auto2.
-    assert (wfB : well_formed B) by wf_auto2.
-
-    eapply MP.
-    2: { apply useBasicReasoning. apply contraposition; wf_auto2. }
-    apply H.
-  Defined.
-  
-  Lemma A_impl_not_not_B {Σ : Signature} Γ A B :
-    well_formed A ->
-    well_formed B ->
-    Γ ⊢i ((A ---> ! !B) ---> (A ---> B))
-    using BasicReasoning.
-  Proof.
-    intros WFA WFB.
-
-    assert (H0 : Γ ⊢i (! !B ---> B) using BasicReasoning).
-    {
-      apply not_not_elim. wf_auto2.
-    }
-
-    assert (H1 : Γ ⊢i ((A ---> ! !B) ---> (! !B ---> B) ---> (A ---> B)) using BasicReasoning).
-    {
-      apply syllogism; wf_auto2.
-    }
-
-    eapply MP.
-    2: { 
-      apply reorder_meta.
-      4: apply H1.
-      all: wf_auto2.
-    }
-    apply H0.
-  Defined.
-
-  Lemma prf_weaken_conclusion {Σ : Signature} Γ A B B' :
-    well_formed A ->
-    well_formed B ->
-    well_formed B' ->
-    Γ ⊢i ((B ---> B') ---> ((A ---> B) ---> (A ---> B')))
-    using BasicReasoning.
-  Proof.
-    intros wfA wfB wfB'.
-    apply reorder_meta;[wf_auto2|wf_auto2|wf_auto2|].
-    apply syllogism; wf_auto2.
-  Defined.
-
-  Lemma prf_weaken_conclusion_meta {Σ : Signature} Γ A B B' (i : ProofInfo) :
-    well_formed A ->
-    well_formed B ->
-    well_formed B' ->
-    Γ ⊢i (B ---> B') using i ->
-    Γ ⊢i ((A ---> B) ---> (A ---> B')) using i.
-  Proof.
-    intros wfA wfB wfB' BimpB'.
-    assert (H1: Γ ⊢i ((A ---> B) ---> (B ---> B') ---> (A ---> B')) using i).
-    {
-      apply useBasicReasoning. apply syllogism; wf_auto2.
-    }
-    apply reorder_meta in H1;[|wf_auto2|wf_auto2|wf_auto2].
-    eapply MP. 2: apply H1. apply BimpB'.
-  Defined.
-
-  Lemma prf_weaken_conclusion_iter {Σ : Signature} Γ l g g'
-          (wfl : Pattern.wf l) (wfg : well_formed g) (wfg' : well_formed g') :
-    Γ ⊢i ((g ---> g') ---> (fold_right patt_imp g l ---> fold_right patt_imp g' l))
-    using BasicReasoning.
-  Proof.
-    induction l.
-    - apply A_impl_A. wf_auto2.
-    - pose proof (wfl' := wfl).
-      apply andb_prop in wfl.
-      fold (map well_formed) in wfl.
-      destruct wfl as [wfa wfl].
-      (* I do not know how to fold it, so I just assert & clear. *)
-      assert (wfl'' : Pattern.wf l) by apply wfl.
-      clear wfl.
-      specialize (IHl wfl'').
-      simpl in *.
-      eapply syllogism_meta.
-      5: eapply prf_weaken_conclusion.
-      4: apply IHl.
-      all: wf_auto2.
-  Defined.
-
-  Lemma prf_weaken_conclusion_iter_meta {Σ : Signature} Γ l g g' (i : ProofInfo):
-    Pattern.wf l ->
-    well_formed g ->
-    well_formed g' ->
-    Γ ⊢i (g ---> g') using i ->
-    Γ ⊢i ((fold_right patt_imp g l) ---> (fold_right patt_imp g' l)) using i.
-  Proof.
-    intros wfl wfg wfg' gimpg'.
-    eapply MP.
-    2: { apply useBasicReasoning. apply prf_weaken_conclusion_iter; wf_auto2. }
-    1: { apply gimpg'. }
-  Defined.
-
-  Lemma prf_weaken_conclusion_iter_meta_meta {Σ : Signature} Γ l g g' (i : ProofInfo):
-    Pattern.wf l ->
-    well_formed g ->
-    well_formed g' ->
-    Γ ⊢i (g ---> g') using i ->
-    Γ ⊢i (fold_right patt_imp g l) using i ->
-    Γ ⊢i (fold_right patt_imp g' l) using i.
-  Proof.
-    intros wfl wfg wfg' gimpg' H.
-    eapply MP.
-    { apply gimpg'. }
-    eapply MP.
-    { apply H. }
-    apply reorder_meta;[wf_auto2|wf_auto2|wf_auto2|].
-    apply useBasicReasoning.
-    apply prf_weaken_conclusion_iter.
-    all: wf_auto2.
-  Defined.
-
-  Lemma prf_weaken_conclusion_meta_meta {Σ : Signature} Γ A B B' (i : ProofInfo) :
-    well_formed A ->
-    well_formed B ->
-    well_formed B' ->
-    Γ ⊢i (B ---> B') using i ->
-    Γ ⊢i (A ---> B) using i ->
-    Γ ⊢i (A ---> B') using i.
-  Proof.
-    intros WFA WFB WFB' H H0.
-    eapply MP. 2: apply prf_weaken_conclusion_meta. 1: apply H0.
-    4: apply H. all: wf_auto2.
-  Defined.
-
-  Lemma prf_strenghten_premise {Σ : Signature} Γ A A' B :
-    well_formed A ->
-    well_formed A' ->
-    well_formed B ->
-    Γ ⊢i ((A' ---> A) ---> ((A ---> B) ---> (A' ---> B))) using BasicReasoning.
-  Proof.
-    intros wfA wfA' wfB.
-    apply syllogism; wf_auto2.
-  Defined.
-
-  Lemma prf_strenghten_premise_iter {Σ : Signature}  Γ l₁ l₂ h h' g :
-    Pattern.wf l₁ -> Pattern.wf l₂ ->
-    well_formed h ->
-    well_formed h' ->
-    well_formed g ->
-    Γ ⊢i (h' ---> h) --->
-        foldr patt_imp g (l₁ ++ h::l₂) --->
-        foldr patt_imp g (l₁ ++ h'::l₂)
-    using BasicReasoning.
-  Proof.
-    intros wfl₁ wfl₂ wfh wfh' wfg.
-    induction l₁.
-    - simpl. apply prf_strenghten_premise. all: wf_auto2.
-    - pose proof (wfal₁ := wfl₁).
-      remember (foldr patt_imp g (h::l₂)) as g1.
-      remember (foldr patt_imp g (h'::l₂)) as g2.
-      unfold Pattern.wf in wfl₁. simpl in wfl₁. apply andb_prop in wfl₁.
-      destruct wfl₁ as [wfa wfl₁].
-      specialize (IHl₁ wfl₁).
-      remember (foldr patt_imp g (l₁ ++ h::l₂)) as b.
-      remember (foldr patt_imp g (l₁ ++ h'::l₂)) as b'.
-
-      assert (prf: Γ ⊢i ((b ---> b') ---> ((a ---> b) ---> (a ---> b'))) using BasicReasoning).
-      { apply prf_weaken_conclusion; subst; wf_auto2. }
-
-      subst.
-      eapply syllogism_meta.
-      5: { apply prf. }
-      4: { apply IHl₁. }
-      all: wf_auto2.
-  Defined.
-
-  Lemma prf_strenghten_premise_meta {Σ : Signature} Γ A A' B (i : ProofInfo) :
-    well_formed A ->
-    well_formed A' ->
-    well_formed B ->
-    Γ ⊢i (A' ---> A) using i ->
-    Γ ⊢i ((A ---> B) ---> (A' ---> B)) using i.
-  Proof.
-    intros wfA wfA' wfB A'impA.
-    assert (H1: Γ ⊢i ((A' ---> A) ---> (A ---> B) ---> (A' ---> B)) using i).
-    {
-      apply useBasicReasoning. apply syllogism; wf_auto2.
-    }
-    eapply MP. 2: apply H1. apply A'impA.
-  Defined.
-
-  Lemma prf_strenghten_premise_meta_meta {Σ : Signature} Γ A A' B (i : ProofInfo) :
-    well_formed A ->
-    well_formed A' ->
-    well_formed B ->
-    Γ ⊢i (A' ---> A) using i ->
-    Γ ⊢i (A ---> B) using i ->
-    Γ ⊢i (A' ---> B) using i.
-  Proof.
-    intros wfA wfA' wfB A'impA AimpB.
-    eapply MP. 2: apply prf_strenghten_premise_meta. 1: apply AimpB.
-    4: apply A'impA. all: wf_auto2.
-  Defined.
-
-  Lemma prf_strenghten_premise_iter_meta {Σ : Signature} Γ l₁ l₂ h h' g (i : ProofInfo) :
-    Pattern.wf l₁ -> Pattern.wf l₂ ->
-    well_formed h ->
-    well_formed h' ->
-    well_formed g ->
-    Γ ⊢i (h' ---> h) using i ->
-    Γ ⊢i foldr patt_imp g (l₁ ++ h::l₂) --->
-         foldr patt_imp g (l₁ ++ h'::l₂)
-    using i.  
-  Proof.
-    intros WFl₁ WFl₂ WFh WFh' WFg H.
-    eapply MP.
-    2: { apply useBasicReasoning. apply prf_strenghten_premise_iter; wf_auto2. }
-    exact H.
-  Defined.
-
-  Lemma prf_strenghten_premise_iter_meta_meta {Σ : Signature} Γ l₁ l₂ h h' g (i : ProofInfo) :
-    Pattern.wf l₁ -> Pattern.wf l₂ ->
-    well_formed h ->
-    well_formed h' ->
-    well_formed g ->
-    Γ ⊢i (h' ---> h) using i ->
-    Γ ⊢i foldr patt_imp g (l₁ ++ h::l₂) using i ->
-    Γ ⊢i foldr patt_imp g (l₁ ++ h'::l₂) using i.  
-  Proof.
-    intros WFl₁ WFl₂ WFh WFh' WFg H H0.
-    eapply MP.
-    2: eapply prf_strenghten_premise_iter_meta.
-    7: eassumption. 1: assumption. all: wf_auto2.
-  Defined.
-
-
-  Local Example example_nested_const {Σ : Signature} Γ a b c:
-    well_formed a ->
-    well_formed b ->
-    well_formed c ->
-    (* like P2 but nested a bit *)
-    Γ ⊢i (a ---> (b ---> (c ---> a)))
-    using BasicReasoning.
-  Proof.
-    intros wfa wfb wfc.
-    assert (H1: Γ ⊢i ((c ---> a) ---> (b ---> (c ---> a))) using BasicReasoning).
+(* This will form a base for the tactic 'exact 0' *)
+Lemma nested_const {Σ : Signature} Γ a l:
+  well_formed a ->
+  Pattern.wf l ->
+  Γ ⊢i (a ---> (fold_right patt_imp a l))
+  using BasicReasoning.
+Proof.
+  intros wfa wfl.
+  induction l; simpl.
+  - apply A_impl_A. exact wfa.
+  - pose proof (wfa0l := wfl).
+    unfold Pattern.wf in wfl. simpl in wfl. apply andb_prop in wfl. destruct wfl as [wfa0 wfl].
+    specialize (IHl wfl).
+    assert (H1 : Γ ⊢i ((foldr patt_imp a l) ---> (a0 ---> (foldr patt_imp a l))) using BasicReasoning).
     {
       apply P1; wf_auto2.
     }
-    assert (H2: Γ ⊢i (a ---> (c ---> a)) using BasicReasoning).
-    { apply P1; wf_auto2. }
+    eapply syllogism_meta.
+    5: apply H1. 4: assumption. all: wf_auto2.
+Defined.
 
-    eapply (syllogism_meta _ _ _ H2 H1).
-    Unshelve. all: wf_auto2.
-  Defined.
+Lemma nested_const_middle {Σ : Signature} Γ a l₁ l₂:
+  well_formed a ->
+  Pattern.wf l₁ ->
+  Pattern.wf l₂ ->
+  Γ ⊢i (fold_right patt_imp a (l₁ ++ a :: l₂))
+  using BasicReasoning.
+Proof.
+  intros wfa wfl₁ wfl₂.
+  induction l₁; simpl.
+  - apply nested_const; wf_auto2.
+  - pose proof (wfa0l₁ := wfl₁).
+    unfold Pattern.wf in wfl₁. simpl in wfl₁. apply andb_prop in wfl₁. destruct wfl₁ as [wfa0 wfl₁].
+    specialize (IHl₁ wfl₁). simpl in IHl₁.
+    eapply MP. 2: apply P1. 1: apply IHl₁. all: wf_auto2.
+Defined.
 
-  (* This will form a base for the tactic 'exact 0' *)
-  Lemma nested_const {Σ : Signature} Γ a l:
-    well_formed a ->
-    Pattern.wf l ->
-    Γ ⊢i (a ---> (fold_right patt_imp a l))
-    using BasicReasoning.
-  Proof.
-    intros wfa wfl.
-    induction l; simpl.
-    - apply A_impl_A. exact wfa.
-    - pose proof (wfa0l := wfl).
-      unfold Pattern.wf in wfl. simpl in wfl. apply andb_prop in wfl. destruct wfl as [wfa0 wfl].
-      specialize (IHl wfl).
-      assert (H1 : Γ ⊢i ((foldr patt_imp a l) ---> (a0 ---> (foldr patt_imp a l))) using BasicReasoning).
-      {
-        apply P1; wf_auto2.
-      }
-      eapply syllogism_meta.
-      5: apply H1. 4: assumption. all: wf_auto2.
-  Defined.
-
-  Lemma nested_const_middle {Σ : Signature} Γ a l₁ l₂:
-    well_formed a ->
-    Pattern.wf l₁ ->
-    Pattern.wf l₂ ->
-    Γ ⊢i (fold_right patt_imp a (l₁ ++ a :: l₂))
-    using BasicReasoning.
-  Proof.
-    intros wfa wfl₁ wfl₂.
-    induction l₁; simpl.
-    - apply nested_const; wf_auto2.
-    - pose proof (wfa0l₁ := wfl₁).
-      unfold Pattern.wf in wfl₁. simpl in wfl₁. apply andb_prop in wfl₁. destruct wfl₁ as [wfa0 wfl₁].
-      specialize (IHl₁ wfl₁). simpl in IHl₁.
-      eapply MP. 2: apply P1. 1: apply IHl₁. all: wf_auto2.
-  Defined.
-
-  Lemma prf_reorder_iter {Σ : Signature} Γ a b g l₁ l₂:
-    well_formed a ->
-    well_formed b ->
-    well_formed g ->
-    Pattern.wf l₁ ->
-    Pattern.wf l₂ ->
-    Γ ⊢i ((fold_right patt_imp g (l₁ ++ [a;b] ++ l₂)) --->
-         (fold_right patt_imp g (l₁ ++ [b;a] ++ l₂)))
-    using BasicReasoning.
-  Proof.
-    intros wfa wfb wfg wfl₁ wfl₂.
-    induction l₁; simpl in *.
-    - apply reorder; wf_auto2.
-    - pose proof (wfa0l₁ := wfl₁).
-      unfold Pattern.wf in wfl₁. apply andb_prop in wfl₁. destruct wfl₁ as [wfa0 wfl₁].
-      specialize (IHl₁ wfl₁).
-      eapply prf_weaken_conclusion_meta.
-      4: apply IHl₁.
-      all: wf_auto2.
-  Defined.
-
-  Lemma prf_reorder_iter_meta {Σ : Signature} Γ a b g l₁ l₂ (i : ProofInfo):
-    well_formed a ->
-    well_formed b ->
-    well_formed g ->
-    Pattern.wf l₁ ->
-    Pattern.wf l₂ ->
-    Γ ⊢i (fold_right patt_imp g (l₁ ++ [a;b] ++ l₂)) using i ->
-    Γ ⊢i (fold_right patt_imp g (l₁ ++ [b;a] ++ l₂)) using i.
-  Proof.
-    (* TODO we should have a function/lemma for creating these "meta" variants. *)
-    intros WFa WFb WFg Wfl1 Wfl2 H.
-    eapply MP.
-    2: { apply useBasicReasoning. apply prf_reorder_iter; wf_auto2. }
-    exact H.
-  Defined.
-  
-  Lemma A_impl_not_not_B_meta {Σ : Signature} Γ A B (i : ProofInfo) :
-    well_formed A ->
-    well_formed B ->
-    Γ ⊢i A ---> ! !B using i ->
-    Γ ⊢i A ---> B using i.
-  Proof.
-    intros WFA WFB H.
-    eapply MP.
-    2: { apply useBasicReasoning. apply A_impl_not_not_B; wf_auto2. }
-    exact H.
-  Defined.
-
-  Lemma pf_conj_elim_l {Σ : Signature} Γ A B :
-    well_formed A ->
-    well_formed B ->
-    Γ ⊢i A and B ---> A using BasicReasoning.
-  Proof.
-    intros WFA WFB. unfold patt_and. unfold patt_not at 1.
-
-    assert (Γ ⊢i (! A ---> (! A or ! B)) using BasicReasoning).
-    { apply disj_left_intro; wf_auto2. }
-
-    assert (Γ ⊢i ((! A or ! B) ---> (! A or ! B ---> ⊥) ---> ⊥) using BasicReasoning).
-    {
-      apply modus_ponens; wf_auto2.
-    }
-    assert (Γ ⊢i (! A ---> ((! A or ! B ---> ⊥) ---> ⊥)) using BasicReasoning).
-    { eapply syllogism_meta. 5: apply H0. 4: apply H. all: wf_auto2. }
-    epose proof (reorder_meta _ _ _ H1).
-    apply A_impl_not_not_B_meta;[wf_auto2|wf_auto2|].
-    apply H2.
-    Unshelve.
+Lemma prf_reorder_iter {Σ : Signature} Γ a b g l₁ l₂:
+  well_formed a ->
+  well_formed b ->
+  well_formed g ->
+  Pattern.wf l₁ ->
+  Pattern.wf l₂ ->
+  Γ ⊢i ((fold_right patt_imp g (l₁ ++ [a;b] ++ l₂)) --->
+       (fold_right patt_imp g (l₁ ++ [b;a] ++ l₂)))
+  using BasicReasoning.
+Proof.
+  intros wfa wfb wfg wfl₁ wfl₂.
+  induction l₁; simpl in *.
+  - apply reorder; wf_auto2.
+  - pose proof (wfa0l₁ := wfl₁).
+    unfold Pattern.wf in wfl₁. apply andb_prop in wfl₁. destruct wfl₁ as [wfa0 wfl₁].
+    specialize (IHl₁ wfl₁).
+    eapply prf_weaken_conclusion_meta.
+    4: apply IHl₁.
     all: wf_auto2.
-  Defined.
+Defined.
 
-  Lemma pf_conj_elim_r {Σ : Signature} Γ A B :
-    well_formed A ->
-    well_formed B ->
-    Γ ⊢i A and B ---> B using BasicReasoning.
-  Proof.
-    intros WFA WFB. unfold patt_and. unfold patt_not at 1.
+Lemma prf_reorder_iter_meta {Σ : Signature} Γ a b g l₁ l₂ (i : ProofInfo):
+  well_formed a ->
+  well_formed b ->
+  well_formed g ->
+  Pattern.wf l₁ ->
+  Pattern.wf l₂ ->
+  Γ ⊢i (fold_right patt_imp g (l₁ ++ [a;b] ++ l₂)) using i ->
+  Γ ⊢i (fold_right patt_imp g (l₁ ++ [b;a] ++ l₂)) using i.
+Proof.
+  (* TODO we should have a function/lemma for creating these "meta" variants. *)
+  intros WFa WFb WFg Wfl1 Wfl2 H.
+  eapply MP.
+  2: { apply useBasicReasoning. apply prf_reorder_iter; wf_auto2. }
+  exact H.
+Defined.
 
-    assert (Γ ⊢i (! B ---> (! A or ! B)) using BasicReasoning).
-    { apply disj_right_intro; wf_auto2. }
+Lemma A_impl_not_not_B_meta {Σ : Signature} Γ A B (i : ProofInfo) :
+  well_formed A ->
+  well_formed B ->
+  Γ ⊢i A ---> ! !B using i ->
+  Γ ⊢i A ---> B using i.
+Proof.
+  intros WFA WFB H.
+  eapply MP.
+  2: { apply useBasicReasoning. apply A_impl_not_not_B; wf_auto2. }
+  exact H.
+Defined.
 
-    assert (Γ ⊢i ((! A or ! B) ---> (! A or ! B ---> ⊥) ---> ⊥) using BasicReasoning).
-    { apply modus_ponens; wf_auto2. }
+Lemma pf_conj_elim_l {Σ : Signature} Γ A B :
+  well_formed A ->
+  well_formed B ->
+  Γ ⊢i A and B ---> A using BasicReasoning.
+Proof.
+  intros WFA WFB. unfold patt_and. unfold patt_not at 1.
 
-    assert (Γ ⊢i (! B ---> ((! A or ! B ---> ⊥) ---> ⊥)) using BasicReasoning).
-    { eapply syllogism_meta. 5: apply H0. 4: apply H. all: wf_auto2. }
-    epose proof (reorder_meta  _ _ _ H1).
-    apply A_impl_not_not_B_meta;[wf_auto2|wf_auto2|].
-    apply H2.
-    Unshelve.
-    all: wf_auto2.
-  Defined.
+  assert (Γ ⊢i (! A ---> (! A or ! B)) using BasicReasoning).
+  { apply disj_left_intro; wf_auto2. }
 
-  Lemma pf_conj_elim_l_meta {Σ : Signature} Γ A B (i : ProofInfo) :
-    well_formed A ->
-    well_formed B ->
-    Γ ⊢i A and B using i ->
-    Γ ⊢i A using i.
-  Proof.
-    intros WFA WFB H.
-    eapply MP.
-    2: { apply useBasicReasoning. apply pf_conj_elim_l. wf_auto2. shelve. }
-    1: apply H.
-    Unshelve. all: wf_auto2.
-  Defined.
-  
-  Lemma pf_conj_elim_r_meta {Σ : Signature} Γ A B (i : ProofInfo) :
-    well_formed A ->
-    well_formed B ->
-    Γ ⊢i A and B using i ->
-    Γ ⊢i B using i.
-  Proof.
-    intros WFA WFB H.
-    eapply MP.
-    2: apply useBasicReasoning; apply pf_conj_elim_r.
-    1: apply H.
-    all: wf_auto2.
-  Defined.
+  assert (Γ ⊢i ((! A or ! B) ---> (! A or ! B ---> ⊥) ---> ⊥) using BasicReasoning).
+  {
+    apply modus_ponens; wf_auto2.
+  }
+  assert (Γ ⊢i (! A ---> ((! A or ! B ---> ⊥) ---> ⊥)) using BasicReasoning).
+  { eapply syllogism_meta. 5: apply H0. 4: apply H. all: wf_auto2. }
+  epose proof (reorder_meta _ _ _ H1).
+  apply A_impl_not_not_B_meta;[wf_auto2|wf_auto2|].
+  apply H2.
+  Unshelve.
+  all: wf_auto2.
+Defined.
 
-  Lemma A_or_notA {Σ : Signature} Γ A :
-    well_formed A ->
-    Γ ⊢i A or ! A using BasicReasoning.
-  Proof.
-    intros wfA.
-    unfold patt_or.
-    apply A_impl_A. wf_auto2.
-  Defined.
+Lemma pf_conj_elim_r {Σ : Signature} Γ A B :
+  well_formed A ->
+  well_formed B ->
+  Γ ⊢i A and B ---> B using BasicReasoning.
+Proof.
+  intros WFA WFB. unfold patt_and. unfold patt_not at 1.
 
-  Lemma P4m_meta {Σ : Signature} (Γ : Theory) (A B : Pattern) (i : ProofInfo) :
-    well_formed A ->
-    well_formed B ->
-    Γ ⊢i A ---> B using i ->
-    Γ ⊢i A ---> !B using i ->
-    Γ ⊢i !A using i.
-  Proof.
-    intros wfA wfB AimpB AimpnB.
-    pose proof (H1 := P4m Γ A B wfA wfB).
-    assert (H2 : Γ ⊢i (A ---> ! B) ---> ! A using i).
-    { eapply MP. 2: { apply useBasicReasoning; apply H1. } exact AimpB. }
-    eapply MP. 2: { apply H2. } exact AimpnB.
-  Defined.
+  assert (Γ ⊢i (! B ---> (! A or ! B)) using BasicReasoning).
+  { apply disj_right_intro; wf_auto2. }
+
+  assert (Γ ⊢i ((! A or ! B) ---> (! A or ! B ---> ⊥) ---> ⊥) using BasicReasoning).
+  { apply modus_ponens; wf_auto2. }
+
+  assert (Γ ⊢i (! B ---> ((! A or ! B ---> ⊥) ---> ⊥)) using BasicReasoning).
+  { eapply syllogism_meta. 5: apply H0. 4: apply H. all: wf_auto2. }
+  epose proof (reorder_meta  _ _ _ H1).
+  apply A_impl_not_not_B_meta;[wf_auto2|wf_auto2|].
+  apply H2.
+  Unshelve.
+  all: wf_auto2.
+Defined.
+
+Lemma pf_conj_elim_l_meta {Σ : Signature} Γ A B (i : ProofInfo) :
+  well_formed A ->
+  well_formed B ->
+  Γ ⊢i A and B using i ->
+  Γ ⊢i A using i.
+Proof.
+  intros WFA WFB H.
+  eapply MP.
+  2: { apply useBasicReasoning. apply pf_conj_elim_l. wf_auto2. shelve. }
+  1: apply H.
+  Unshelve. all: wf_auto2.
+Defined.
+
+Lemma pf_conj_elim_r_meta {Σ : Signature} Γ A B (i : ProofInfo) :
+  well_formed A ->
+  well_formed B ->
+  Γ ⊢i A and B using i ->
+  Γ ⊢i B using i.
+Proof.
+  intros WFA WFB H.
+  eapply MP.
+  2: apply useBasicReasoning; apply pf_conj_elim_r.
+  1: apply H.
+  all: wf_auto2.
+Defined.
+
+Lemma A_or_notA {Σ : Signature} Γ A :
+  well_formed A ->
+  Γ ⊢i A or ! A using BasicReasoning.
+Proof.
+  intros wfA.
+  unfold patt_or.
+  apply A_impl_A. wf_auto2.
+Defined.
+
+Lemma P4m_meta {Σ : Signature} (Γ : Theory) (A B : Pattern) (i : ProofInfo) :
+  well_formed A ->
+  well_formed B ->
+  Γ ⊢i A ---> B using i ->
+  Γ ⊢i A ---> !B using i ->
+  Γ ⊢i !A using i.
+Proof.
+  intros wfA wfB AimpB AimpnB.
+  pose proof (H1 := P4m Γ A B wfA wfB).
+  assert (H2 : Γ ⊢i (A ---> ! B) ---> ! A using i).
+  { eapply MP. 2: { apply useBasicReasoning; apply H1. } exact AimpB. }
+  eapply MP. 2: { apply H2. } exact AimpnB.
+Defined.
 
 Lemma MLGoal_exactn {Σ : Signature}
   (Γ : Theory)
@@ -1360,18 +1361,6 @@ Proof.
   mlApply "H3".
   mlApply "H0".
   mlExact "H4".
-Defined.
-
-Lemma prf_add_assumption {Σ : Signature} Γ a b i :
-  well_formed a ->
-  well_formed b ->
-  Γ ⊢i b using i ->
-  Γ ⊢i (a ---> b) using i.
-Proof.
-  intros wfa wfb H.
-  eapply MP.
-  { apply H. }
-  { useBasicReasoning. apply P1; wf_auto2. }
 Defined.
 
 Lemma prf_impl_distr_meta {Σ : Signature} Γ a b c i:
@@ -2899,7 +2888,7 @@ Ltac _mlApplyMetaIn t name :=
   let ff := ltac2:(t' name' |- mlApplyMetaIn (Option.get (Ltac1.to_constr(t'))) (Option.get (Ltac1.to_constr(name')))) in
   ff t name
 .
-  
+
 Tactic Notation "mlApplyMeta" constr(t) :=
   _mlApplyMeta t.
 
@@ -2996,7 +2985,7 @@ Proof.
   }
 
   eapply cast_proof_ml_hyps.
-  {  
+  {
     replace (l₁ ++ (mkNH _ nxy (x and y)) :: l₂) with ((l₁++ [mkNH _ nxy (x and y)]) ++ l₂).
     2: { rewrite -app_assoc. reflexivity. }
     rewrite take_app. rewrite drop_app. reflexivity.
@@ -3935,20 +3924,6 @@ Proof.
   mlExactMeta (top_holds Γ).
 Defined.
 
-Lemma MLGoal_Exfalso {Σ : Signature} : forall Γ l g i,
-  mkMLGoal Σ Γ l Bot i ->
-  mkMLGoal Σ Γ l g i.
-Proof.
-  intros Γ l g i H WFg WFl.
-  unfold of_MLGoal in *; simpl in *.
-  apply H in WFl as WFl'; auto.
-  eapply prf_weaken_conclusion_iter_meta_meta. 5: exact WFl'.
-  all: wf_auto2.
-  gapply bot_elim. apply pile_basic_generic'. auto.
-Defined.
-
-Tactic Notation "mlExfalso" := apply MLGoal_Exfalso.
-
 Local Example exfalso_test {Σ : Signature} p Γ i :
   well_formed p ->
   Γ ⊢i p and ! p ---> Top using i.
@@ -3957,7 +3932,7 @@ Proof.
   { wf_auto2. }
   mlIntro "H".
   mlDestructAnd "H" as "H0" "H1".
-  mlExfalso.
+  mlExFalso.
   mlApply "H1".
   mlExact "H0".
 Defined.
